Added 'proof' that Init_ex can't handle InitializedDigestSet

dig/abstractspec_digests.v
@@ -381,6 +381,19 @@ Definition OPENSSL_memset_SPEC := DECLARE _OPENSSL_memset
            | memsetNonnull sh => data_at sh (tarray tuchar n) (list_repeat (Z.to_nat n) (Vint c)) p
            end).
 
+Parameter ERR: val -> mpred. 
+Definition OPENSSL_PUT_ERROR_SPEC := DECLARE _ERR_put_error
+  WITH a1:val, a2:val, a3:val, ep:val, a5:val
+  PRE [ 1%positive OF tint, 
+        2%positive OF tint, 3%positive OF tint, 
+        4%positive OF (tptr tschar), 5%positive OF tuint ]
+      PROP() 
+      LOCAL (temp 1%positive a1; temp 2%positive a2; temp 3%positive a3; 
+             temp 4%positive ep; temp 5%positive a5)
+      SEP (ERR ep)
+  POST [ tvoid ]
+    PROP () LOCAL () SEP (ERR ep).
+
 Definition GprogMemset: funspecs := [OPENSSL_memset_SPEC; memset_spec].
 Lemma body_OPENSSL_mmemset_SPEC: semax_body Vprog GprogMemset f_OPENSSL_memset OPENSSL_memset_SPEC.
 Proof.
@@ -481,11 +494,701 @@ Definition mddata_of_ctx (v:reptype (Tstruct _env_md_ctx_st noattr)) :=
     (type, (mddata, pv)) => mddata
   end.
 
+(****** Used in the specs of the four Digest Operation Accessors. *******)
+(*nonnull node*)
+Definition EVP_MD_CTX_NNnode (sh:share) (vals:val*(val*(val*val))) (p:val):mpred :=
+  match vals with (d, (mddata, (pctx, pctxops))) =>
+  !!(is_pointer_or_null d /\ is_pointer_or_null mddata) &&
+  data_at sh (Tstruct _env_md_ctx_st noattr) (d,(mddata,(pctx, pctxops))) p
+  end.
+
+Lemma EVP_MD_CTX_NNnode_isptr sh vals p:
+  EVP_MD_CTX_NNnode sh vals p |-- !!(isptr p).
+Proof.
+  unfold EVP_MD_CTX_NNnode. destruct vals as [d [mdd [pc pcops]]]. normalize.
+  rewrite data_at_isptr. entailer!.
+Qed.
+Lemma EVP_MD_CTX_NNnode_isptr' sh vals p:
+  EVP_MD_CTX_NNnode sh vals p  = (!!(isptr p) &&  EVP_MD_CTX_NNnode sh vals p).
+Proof.
+  apply pred_ext; [ entailer; apply EVP_MD_CTX_NNnode_isptr | entailer!].
+Qed.
+
+(*a possibly null node*)
+Definition EVP_MD_CTX_node sh (vals:val*(val*(val*val))) (p:val):mpred :=
+ (!!(p = nullval) && emp) || EVP_MD_CTX_NNnode sh vals p.
+
+Lemma EVP_MD_CTX_node_null sh vals: EVP_MD_CTX_node sh vals nullval |-- emp.
+Proof. apply orp_left; [| rewrite EVP_MD_CTX_NNnode_isptr']; normalize. Qed.
+
+Hint Resolve EVP_MD_CTX_node_null: cancel.
+
+(*nonnull node*)
+Definition EVP_MD_NNnode (sh:share) (vals:reptype (Tstruct _env_md_st noattr)) (p:val):mpred :=
+  !!(readable_share sh) &&
+  data_at sh (Tstruct _env_md_st noattr) vals p.
+
+Lemma EVP_MD_NNnode_isptr sh vals p: EVP_MD_NNnode sh vals p |-- !!(isptr p).
+Proof.
+  unfold EVP_MD_NNnode. destruct vals. normalize.
+  rewrite data_at_isptr. entailer!.
+Qed.
+
+Lemma EVP_MD_NNnode_isptr' sh vals p:
+  EVP_MD_NNnode sh vals p  = (!!(isptr p) &&  EVP_MD_NNnode sh vals p).
+Proof.
+  apply pred_ext; [ entailer; apply EVP_MD_NNnode_isptr | entailer!].
+Qed.
+
+Lemma EVP_MD_NNnode_validptr sh vals p:  EVP_MD_NNnode sh vals p |-- valid_pointer p.
+Proof. unfold EVP_MD_NNnode. entailer!. Qed.
+
+(*a possibly null node*)
+Definition EVP_MD_node (vals:reptype (Tstruct _env_md_st noattr))(p:val):mpred :=
+ (!!(p = nullval) && emp) || (EX sh:_, EVP_MD_NNnode sh vals p).
+
+Lemma EVP_MD_node_null vals: EVP_MD_node vals nullval |-- emp.
+Proof. apply orp_left; [| Intros sh; rewrite EVP_MD_NNnode_isptr' ]; normalize. Qed.
+
+Hint Resolve EVP_MD_node_null: cancel.
+
+Lemma EVP_MD_node_validptr vals p:  EVP_MD_node vals p |-- valid_pointer p.
+Proof. unfold EVP_MD_node.
+  apply orp_left; normalize. apply valid_pointer_null.
+  apply EVP_MD_NNnode_validptr. 
+Qed.
+
+Definition get_type (vals:reptype (Tstruct _env_md_st noattr)):=
+  match vals with
+    (type, (mds, (flags, (ini, (upd, (fin, (blsize, ctxsize))))))) => type
+  end.
+Definition get_mdsize (vals:reptype (Tstruct _env_md_st noattr)):=
+  match vals with
+    (type, (mds, (flags, (ini, (upd, (fin, (blsize, ctxsize))))))) => mds
+  end.
+Definition get_iniptr (vals:reptype (Tstruct _env_md_st noattr)):=
+  match vals with
+    (type, (mds, (flags, (ini, (upd, (fin, (blsize, ctxsize))))))) => ini
+  end.
+Definition get_updptr (vals:reptype (Tstruct _env_md_st noattr)):=
+  match vals with
+    (type, (mds, (flags, (ini, (upd, (fin, (blsize, ctxsize))))))) => upd
+  end.
+Definition get_finptr (vals:reptype (Tstruct _env_md_st noattr)):=
+  match vals with
+    (type, (mds, (flags, (ini, (upd, (fin, (blsize, ctxsize))))))) => fin
+  end.
+Definition get_blsize (vals:reptype (Tstruct _env_md_st noattr)):=
+  match vals with
+    (type, (mds, (flags, (ini, (upd, (fin, (blsize, ctxsize))))))) => blsize
+  end.
+Definition get_ctxsize (vals:reptype (Tstruct _env_md_st noattr)):=
+  match vals with
+    (type, (mds, (flags, (ini, (upd, (fin, (blsize, ctxsize))))))) => ctxsize
+  end.
+
+Lemma Valeq_Vint {A} i j (a b:A):
+      (if Val.eq (Vint i) (Vint j) then a else b) =
+      (if Int.eq i j then a else b).
+Proof. 
+ remember (Int.eq i j). destruct b0.
++ rewrite ( binop_lemmas2.int_eq_true _ _ Heqb0). rewrite if_true; trivial.
++ remember (Val.eq (Vint i )(Vint j)) as d.
+  destruct d; trivial.
+  inversion e; subst; simpl in *.
+  specialize (int_eq_false_e j j); intuition.
+Qed. 
+
+Module Type EVP_MD_CTX_Protocol_TP.
+Parameter MDCTXInitialized: val -> mpred.
+Parameter MDCTXAllocated: val -> mpred.
+
+(*Propose to Adam that this be eliminated - it's needed in 3 places*)
+Parameter MDCTXInitializedDigestSet: val -> val -> mpred.
+
+Axiom MDCTXAllocated_valid_ptr: forall p, MDCTXAllocated p |-- valid_pointer p.
+
+Axiom MDCTXInitialized_MDCTXAllocated: forall p, MDCTXInitialized p|-- MDCTXAllocated p.
+
+Axiom MDCTXInitializedDigestSet_MDCTXAllocated: forall t p, MDCTXInitializedDigestSet t p|-- MDCTXAllocated p.
+
+Axiom MDCTXInitialized_valid_ptr: forall p, MDCTXInitialized p |-- valid_pointer p.
+
+Axiom MDCTXInitializedDigestSet_valid_ptr: forall t p, MDCTXInitializedDigestSet t p |-- valid_pointer p.
+
+Axiom MDCTXAllocated_isptr: forall p, MDCTXAllocated p |-- !! isptr p.
+
+Axiom MDCTXInitialized_isptr: forall p, MDCTXInitialized p |-- !! isptr p.
+
+Axiom MDCTXInitializedDigestSet_isptr: forall t p, MDCTXInitializedDigestSet t p |-- !! isptr p.
+
+Axiom MDCTXAllocated_isptr': forall p, MDCTXAllocated p = (!!isptr p) && MDCTXAllocated p.
+
+Axiom MDCTXInitialized_isptr': forall p, MDCTXInitialized p = (!! isptr p) && MDCTXInitialized p.
+
+Axiom MDCTXInitializedDigestSet_isptr': forall t p, MDCTXInitializedDigestSet t p = (!! isptr p) && MDCTXInitializedDigestSet t p.
+
+Definition EVP_MD_CTX_init_SPEC := DECLARE _EVP_MD_CTX_init
+   WITH ctx:val
+   PRE [ _ctx OF tptr (Tstruct _env_md_ctx_st noattr) ]
+       PROP () LOCAL (temp _ctx ctx) SEP (MDCTXAllocated ctx)
+   POST [ tvoid ]
+       PROP () LOCAL () SEP (MDCTXInitialized ctx).
+
+Definition EVP_MD_CTX_create_SPEC := DECLARE _EVP_MD_CTX_create
+   WITH ctx:val
+   PRE [ ]
+       PROP () LOCAL ( ) SEP ()
+   POST [ tptr (Tstruct _env_md_ctx_st noattr) ]
+     EX ctx:val,
+       PROP ()
+       LOCAL (temp ret_temp ctx)
+       SEP ((!!(ctx=nullval) && emp) || MDCTXInitialized ctx).
+
+Definition Gprog_EVPMDCTX_1 : funspecs :=
+  (*FAILS TO TERMINATE: ltac:(with_library prog [EVP_MD_type_SPEC]). *)
+  [EVP_MD_CTX_create_SPEC; EVP_MD_CTX_init_SPEC; OPENSSL_memset_SPEC; OPENSSL_malloc_SPEC].
+
+Axiom body_EVP_MD_CTX_init: semax_body Vprog Gprog_EVPMDCTX_1 f_EVP_MD_CTX_init EVP_MD_CTX_init_SPEC.
+
+Axiom body_EVP_MD_CTX_create: semax_body Vprog Gprog_EVPMDCTX_1 f_EVP_MD_CTX_create EVP_MD_CTX_create_SPEC.
+
+(*According to digest.h, EVP_MD_CTX_md may be invoked even if no digest has not been set, 
+  returning null in this case. The other 3 functions are specified to crash in such a 
+  situation - we hence strengthen the precondition to rule out these situations*)
+Definition EVP_MD_CTX_md_SPEC := DECLARE _EVP_MD_CTX_md
+  WITH ctx:val, sh:share, d:val, x:val * (val * val)
+  PRE [ _ctx OF (tptr (Tstruct _env_md_ctx_st noattr)) ]
+      PROP (readable_share sh)
+      LOCAL (temp _ctx ctx)
+      SEP (EVP_MD_CTX_node sh (d, x) ctx)
+  POST [ tptr (Tstruct _env_md_st noattr) ]
+       PROP ()
+       LOCAL (temp ret_temp (if Val.eq ctx nullval then nullval else d))
+       SEP (EVP_MD_CTX_node sh (d, x) ctx).
+
+Definition EVP_MD_CTX_size_SPEC := DECLARE _EVP_MD_CTX_size
+  WITH ctx:val, sh:share, r:EVP_MD_record, d:val, x:val * (val * val)
+  PRE [ _ctx OF (tptr (Tstruct _env_md_ctx_st noattr)) ]
+      PROP (readable_share sh)
+      LOCAL (temp _ctx ctx)
+      SEP (EVP_MD_CTX_NNnode sh (d, x) ctx;  EVP_MD_rep r d)
+  POST [ tptr (Tstruct _env_md_st noattr) ]
+       PROP (readable_share sh)
+       LOCAL (temp ret_temp (Vint (Int.repr (EVP_MD_rec_md_size r))))
+       SEP (EVP_MD_CTX_NNnode sh (d, x) ctx;  EVP_MD_rep r d).
+
+Definition EVP_MD_CTX_block_size_SPEC := DECLARE _EVP_MD_CTX_block_size
+  WITH ctx:val, sh:share, r:EVP_MD_record, d:val, x:val * (val * val)
+  PRE [ _ctx OF (tptr (Tstruct _env_md_ctx_st noattr)) ]
+      PROP (readable_share sh)
+      LOCAL (temp _ctx ctx)
+      SEP (EVP_MD_CTX_NNnode sh (d, x) ctx;  EVP_MD_rep r d)
+  POST [ tptr (Tstruct _env_md_st noattr) ]
+       PROP (readable_share sh)
+       LOCAL (temp ret_temp (Vint (Int.repr (EVP_MD_rec_block_size r))))
+       SEP (EVP_MD_CTX_NNnode sh (d, x) ctx;  EVP_MD_rep r d).
+
+Definition EVP_MD_CTX_type_SPEC := DECLARE _EVP_MD_CTX_type
+  WITH ctx:val, sh:share, r:EVP_MD_record, d:val, x:val * (val * val)
+  PRE [ _ctx OF (tptr (Tstruct _env_md_ctx_st noattr)) ]
+      PROP (readable_share sh)
+      LOCAL (temp _ctx ctx)
+      SEP (EVP_MD_CTX_NNnode sh (d, x) ctx;  EVP_MD_rep r d)
+  POST [ tptr (Tstruct _env_md_st noattr) ]
+       PROP ()
+       LOCAL (temp ret_temp (Vint (Int.repr (NID_of_DigestNID (EVP_MD_rec_type r)))))
+       SEP (EVP_MD_CTX_NNnode sh (d, x) ctx;  EVP_MD_rep r d).
+
+Definition Gprog_DigAccessOps : funspecs :=
+  (*FAILS TO TERMINATE: ltac:(with_library prog [EVP_MD_type_SPEC]). *)
+  [EVP_MD_block_size_SPEC; EVP_MD_type_SPEC; EVP_MD_size_SPEC  (*called*);
+   EVP_MD_CTX_md_SPEC; EVP_MD_CTX_size_SPEC; EVP_MD_CTX_block_size_SPEC; EVP_MD_CTX_type_SPEC].
+
+Axiom body_EVP_MD_CTX_block_size: semax_body Vprog Gprog_DigAccessOps f_EVP_MD_CTX_block_size EVP_MD_CTX_block_size_SPEC.
+Axiom body_EVP_MD_CTX_type: semax_body Vprog Gprog_DigAccessOps f_EVP_MD_CTX_type EVP_MD_CTX_type_SPEC.
+Axiom body_EVP_MD_CTX_size: semax_body Vprog Gprog_DigAccessOps f_EVP_MD_CTX_size EVP_MD_CTX_size_SPEC.
+Axiom body_EVP_MD_CTX_md: semax_body Vprog Gprog_DigAccessOps f_EVP_MD_CTX_md EVP_MD_CTX_md_SPEC.
+
+Definition Gprog_cleanup : funspecs :=
+  (*FAILS TO TERMINATE: ltac:(with_library prog [EVP_MD_type_SPEC]). *)
+  [OPENSSL_cleanse_SPEC; OPENSSL_free_SPEC; EVP_MD_CTX_init_SPEC].
+(*
+Parameter struct_of_nid: int -> option type.
+Parameter DigestRep: forall (t:type) (v:reptype t) (data:list Z), Prop. (*should generalize s256_relate*)
+Parameter DigestRepNil: forall t, DigestRep t (default_val t) [].
+*)
+Parameter MDCTXConfigured: forall (nid ctxsz:int) (d p:val), mpred.
+Parameter MDCTXHashed: forall (nid ctxsz:int) (data:list Z) (d p:val), mpred.
+Parameter MDCTXFinished: forall (nid ctxsz:int) (d p:val), mpred.
+
+Axiom MDCTXConfigured_valid_ptr: forall nid ctxsz d p, MDCTXConfigured nid ctxsz d p |-- valid_pointer p.
+Axiom MDCTXConfigured_isptr: forall nid ctxsz d p, MDCTXConfigured ctxsz nid d p |-- !! isptr p.
+Axiom MDCTXConfigured_isptr': forall nid ctxsz d p, MDCTXConfigured nid ctxsz d p = (!!isptr p) && MDCTXConfigured nid ctxsz d p.
+
+Axiom MDCTXHashed_valid_ptr: forall nid ctxsz data d p, MDCTXHashed nid ctxsz data d p |-- valid_pointer p.
+Axiom MDCTXHashed_isptr: forall nid ctxsz data d p, MDCTXHashed nid ctxsz data d p |-- !! isptr p.
+Axiom MDCTXHashed_isptr': forall nid ctxsz data d p,
+      MDCTXHashed nid ctxsz data d p = (!!isptr p) && MDCTXHashed nid ctxsz data d p.
+
+Axiom MDCTXHashed_MDCTXConfigured: forall nid ctxsz data d p, MDCTXHashed nid ctxsz data d p |-- MDCTXConfigured nid ctxsz d p.
+Axiom MDCTXConfigured_MDCTXHashed: forall nid ctxsz d p, MDCTXConfigured nid ctxsz d p |-- MDCTXHashed nid ctxsz nil d p.
+
+Axiom MDCTXFinished_valid_ptr: forall nid ctxsz d p, MDCTXFinished nid ctxsz d p |-- valid_pointer p.
+Axiom MDCTXFinished_isptr: forall nid ctxsz d p, MDCTXFinished nid ctxsz d p |-- !! isptr p.
+Axiom MDCTXFinished_isptr': forall nid ctxsz d p,
+      MDCTXFinished nid ctxsz d p = (!!isptr p) && MDCTXFinished nid ctxsz d p.
+
+Definition MDCTXHashedOrFinished nid ctxsz d p: mpred :=
+  (EX data:_, MDCTXHashed nid ctxsz (map Int.unsigned data) d p) || MDCTXFinished nid ctxsz d p.
+
+Axiom MDCTXHashedOrFinished_valid_ptr: forall nid ctxsz d p, MDCTXHashedOrFinished nid ctxsz d p |-- valid_pointer p.
+Axiom MDCTXHashedOrFinished_isptr: forall nid ctxsz d p, MDCTXHashedOrFinished nid ctxsz d p |-- !!(isptr p).
+Axiom MDCTXHashedOrFinished_isptr': forall nid ctxsz d p,
+      MDCTXHashedOrFinished nid ctxsz d p = !!(isptr p) && MDCTXHashedOrFinished nid ctxsz d p.
+
+(*Not exposed
+Axiom MDCTXHashedOrFinished_MDCTXFinished: forall nid ctxsz d p,
+      MDCTXHashedOrFinished nid ctxsz d p = MDCTXFinished nid ctxsz d p.
+
+Lemma MDCTXFinished_MDCTXConfigured nid ctxsz d p:, MDCTXFinished nid ctxsz d p = MDCTXConfigured nid ctxsz d p.
+Proof. unfold MDCTXFinished, MDCTXConfigured, postInit; apply pred_ext; Intros md t; Exists md t; entailer!. Qed.
+
+Lemma MDCTXHashed_MDCTXFinished nid ctxsz data d p, MDCTXHashed nid ctxsz data d p |-- MDCTXFinished nid ctxsz d p.
+Proof. unfold MDCTXFinished, MDCTXHashed; Intros md t v. Exists md t; entailer!. Qed.
+*)
+
+Inductive EVP_MD_CTX_cleanup_case :=
+  ClInitialized: EVP_MD_CTX_cleanup_case
+| ClInitializedDigestSet: forall (d:val) (dsh:share) (vals:reptype (Tstruct _env_md_st noattr)), EVP_MD_CTX_cleanup_case (*Talk with Adam to allow removal of this*)
+| ClConfiguredOrFinished: forall (dsh:share) (vals:reptype (Tstruct _env_md_st noattr)) (d:val), EVP_MD_CTX_cleanup_case.
+
+Definition EVP_MD_CTX_cleanup_pre (c:EVP_MD_CTX_cleanup_case) (ctx:val) : mpred :=
+  match c with
+   ClInitialized => MDCTXInitialized ctx
+ | ClInitializedDigestSet t tsh vals => EX ctxsz:int, 
+     !!(get_ctxsize vals = Vint ctxsz /\ Int.eq ctxsz Int.zero = false)
+     && MDCTXInitializedDigestSet t ctx * EVP_MD_NNnode tsh vals t
+ | ClConfiguredOrFinished dsh vals d => 
+     EX nid:int, EX ctxsz:int, 
+     !!(get_ctxsize vals = Vint ctxsz /\ get_type vals = Vint nid)
+     && (MDCTXConfigured nid ctxsz d ctx || MDCTXFinished nid ctxsz d ctx) * EVP_MD_NNnode dsh vals d
+end.
+
+Definition EVP_MD_CTX_cleanup_post (c:EVP_MD_CTX_cleanup_case) (ctx:val) : mpred :=
+  match c with
+   ClInitialized => MDCTXInitialized ctx
+ | ClInitializedDigestSet t tsh vals => MDCTXInitialized ctx * EVP_MD_NNnode tsh vals t
+ | ClConfiguredOrFinished dsh vals d => MDCTXInitialized ctx * EVP_MD_NNnode dsh vals d
+end.
+
+Definition EVP_MD_CTX_cleanup_SPEC := DECLARE _EVP_MD_CTX_cleanup
+  WITH ctx:val, c:EVP_MD_CTX_cleanup_case
+  PRE [ _ctx OF (tptr (Tstruct _env_md_ctx_st noattr)) ]
+      PROP () LOCAL (temp _ctx ctx)
+      SEP (EVP_MD_CTX_cleanup_pre c ctx)
+  POST [ tint ]
+       PROP () LOCAL (temp ret_temp (Vint (Int.one)))
+       SEP (EVP_MD_CTX_cleanup_post c ctx).
+
+Axiom body_EVP_MD_CTX_cleanup: semax_body Vprog Gprog_cleanup f_EVP_MD_CTX_cleanup EVP_MD_CTX_cleanup_SPEC.
+
+Parameter preInit: Z -> val -> mpred.
+Parameter memblock_preInit: forall i m, memory_block Tsh i m |-- preInit i m.
+
+Parameter postInit: forall (nid:int) (ctxsz:Z) (p:val), mpred.
+
+Definition ini_spec:funspec :=
+  WITH ctx: val, sh:share, 
+       CTX: reptype (Tstruct _env_md_ctx_st noattr),
+       dsh: share, dvals: reptype (Tstruct _env_md_st noattr), ctxsz:int, nid:int
+  PRE [ 1%positive OF tptr (Tstruct _env_md_ctx_st noattr)]
+          PROP (writable_share sh; readable_share dsh; get_ctxsize dvals = Vint ctxsz;
+                get_type dvals = Vint nid)
+          LOCAL (temp 1%positive ctx)
+          SEP (data_at sh (Tstruct _env_md_ctx_st noattr) CTX ctx;
+               preInit (Int.unsigned ctxsz) (mddata_of_ctx CTX);
+               data_at dsh (Tstruct _env_md_st noattr) dvals (type_of_ctx CTX))
+  POST [ tvoid ]
+          PROP() LOCAL () 
+          SEP(data_at sh (Tstruct _env_md_ctx_st noattr) CTX ctx;
+              postInit nid (Int.unsigned ctxsz) (mddata_of_ctx CTX);
+              data_at dsh (Tstruct _env_md_st noattr) dvals (type_of_ctx CTX)).
+
+Inductive EVP_DigestInit_ex_case :=
+  Initialized: forall (tsh:share) (vals:reptype (Tstruct _env_md_st noattr)), EVP_DigestInit_ex_case
+(*Adam: InitiatlizedDigestSet case fails, if ctx->digest = type*)
+| HashFinishedEQ: forall (tsh:share) (vals:reptype (Tstruct _env_md_st noattr)), EVP_DigestInit_ex_case
+| HashFinishedNEQ: forall (tsh dsh:share) (vals dvals:reptype (Tstruct _env_md_st noattr)) (d:val), EVP_DigestInit_ex_case.
+
+(*
+Axiom Adam1: forall ctx t, 
+  field_at Tsh (Tstruct _env_md_ctx_st noattr) [] (t, (nullval, (nullval, nullval))) ctx
+  |-- data_at Tsh (Tstruct _env_md_ctx_st noattr) (nullval, (nullval, (nullval, nullval))) ctx.
+*)
+
+Definition EVP_DigestInit_ex_pre (c:EVP_DigestInit_ex_case) (t ctx:val): mpred :=
+  match c with
+    Initialized tsh vals =>
+      EX nid:int, EX ctxsz: int, 
+      !!(get_ctxsize vals = Vint ctxsz /\ get_type vals = Vint nid /\
+         4 <= Int.unsigned ctxsz <= Int.max_unsigned /\ is_pointer_or_null (get_iniptr vals) )
+      && EVP_MD_NNnode tsh vals t * func_ptr' ini_spec (get_iniptr vals) *
+         MDCTXInitialized ctx
+  | HashFinishedEQ tsh vals => EVP_MD_NNnode tsh vals t * func_ptr' ini_spec (get_iniptr vals) *
+      EX nid: int, EX ctxsz: int,
+         !!(get_ctxsize vals = Vint ctxsz /\ get_type vals = Vint nid /\
+            4 < Int.unsigned ctxsz <= Int.max_unsigned /\ is_pointer_or_null (get_iniptr vals))
+         && (MDCTXFinished nid ctxsz t ctx || EX data:_, MDCTXHashed nid ctxsz data t ctx)
+  | HashFinishedNEQ tsh dsh vals dvals d => 
+      EX nid:int, EX ctxsz:int,
+      !!(get_ctxsize vals = Vint ctxsz /\ get_type vals = Vint nid /\
+         4 <= Int.unsigned ctxsz <= Int.max_unsigned /\ is_pointer_or_null (get_iniptr vals) )
+      &&
+      EVP_MD_NNnode tsh vals t * func_ptr' ini_spec (get_iniptr vals) * EVP_MD_NNnode dsh dvals d *
+      EX nid': int, EX ctxsz': int,
+         !!(d<>t /\ get_ctxsize dvals = Vint ctxsz' /\ get_type dvals = Vint nid' /\
+            0 < Int.unsigned ctxsz' <= Int.max_unsigned)
+         && (MDCTXFinished nid' ctxsz' d ctx || EX data:_, MDCTXHashed nid' ctxsz' data d ctx)
+end.
+
+Definition EVP_DigestInit_ex_post (c:EVP_DigestInit_ex_case) (t ctx rv:val): mpred :=
+  match c with
+    Initialized tsh vals => EVP_MD_NNnode tsh vals t * func_ptr' ini_spec (get_iniptr vals) * 
+          (    (!!(rv=Vzero) && MDCTXInitializedDigestSet t ctx)
+            || (!!(rv=Vone) && EX nid: int, EX ctxsz: int,
+                !!(get_ctxsize vals = Vint ctxsz /\ get_type vals = Vint nid) 
+                && MDCTXConfigured nid ctxsz t ctx) )
+  | HashFinishedEQ tsh vals => !!(rv=Vone) &&
+      EX nid: int, EX ctxsz: int,
+         !!(get_ctxsize vals = Vint ctxsz /\ get_type vals = Vint nid) 
+         && MDCTXConfigured nid ctxsz t ctx * EVP_MD_NNnode tsh vals t * func_ptr' ini_spec (get_iniptr vals)
+  | HashFinishedNEQ tsh dsh vals dvals d => 
+      EVP_MD_NNnode tsh vals t * func_ptr' ini_spec (get_iniptr vals) * EVP_MD_NNnode dsh dvals d *
+        (   (!!(rv=Vzero) && MDCTXInitializedDigestSet t ctx)
+         || (!!(rv=Vone) && EX nid: int, EX ctxsz: int,
+             !!(get_ctxsize vals = Vint ctxsz /\ get_type vals = Vint nid) && MDCTXConfigured nid ctxsz t ctx))
+end.
+
+Definition EVP_DigestInit_ex_SPEC := DECLARE _EVP_DigestInit_ex
+  WITH ep: val, ctx:val, t:val, e:val, c:EVP_DigestInit_ex_case
+  PRE [ _ctx OF tptr (Tstruct _env_md_ctx_st noattr), 
+        _type OF tptr (Tstruct _env_md_st noattr),
+        _engine OF tptr (Tstruct _engine_st noattr) ]
+      PROP ()
+      LOCAL (gvar ___stringlit_1 ep; temp _type t; temp _ctx ctx; temp _engine e)
+      SEP (ERR ep; EVP_DigestInit_ex_pre c t ctx)
+  POST [ tint] EX rv:_,
+       PROP () LOCAL (temp ret_temp rv)
+       SEP (ERR ep; EVP_DigestInit_ex_post c t ctx rv). 
+
+Definition Gprog_DigestInit_ex : funspecs :=
+  [OPENSSL_PUT_ERROR_SPEC; OPENSSL_free_SPEC; OPENSSL_malloc_SPEC].
+
+Axiom body_DigestInit_ex: semax_body Vprog Gprog_DigestInit_ex f_EVP_DigestInit_ex EVP_DigestInit_ex_SPEC.
+
+Definition EVP_DigestInit_SPEC := DECLARE _EVP_DigestInit
+  WITH ep: val, ctx:val, t:val, tsh:share, 
+       vals:reptype (Tstruct _env_md_st noattr), ctxsz:int, nid:int
+  PRE [ _ctx OF tptr (Tstruct _env_md_ctx_st noattr), 
+        _type OF tptr (Tstruct _env_md_st noattr) ]
+      PROP (get_ctxsize vals = Vint ctxsz;
+            4 <= Int.unsigned ctxsz <= Int.max_unsigned;
+            is_pointer_or_null (get_iniptr vals); 
+            get_type vals = Vint nid)
+      LOCAL (gvar ___stringlit_1 ep; temp _type t; temp _ctx ctx)
+      SEP (MDCTXAllocated ctx; ERR ep; EVP_MD_NNnode tsh vals t;
+           func_ptr' ini_spec (get_iniptr vals))
+  POST [ tint] EX rv:_,
+       PROP ()
+       LOCAL (temp ret_temp rv)
+       SEP ((!!(rv=Vzero) && MDCTXInitializedDigestSet t ctx)
+            || (!!(rv=Vone) && MDCTXConfigured nid ctxsz t ctx);
+            ERR ep; EVP_MD_NNnode tsh vals t; func_ptr' ini_spec (get_iniptr vals)).
+
+Definition Gprog_DigestInit : funspecs :=
+  (*FAILS TO TERMINATE: ltac:(with_library prog [EVP_MD_type_SPEC]). *)
+  [EVP_DigestInit_ex_SPEC; EVP_MD_CTX_init_SPEC].
+
+Axiom body_DigestInit: semax_body Vprog Gprog_DigestInit f_EVP_DigestInit EVP_DigestInit_SPEC.
+
+Definition upd_spec:funspec :=
+  WITH ctx: val, nid:int, ctxsz:int, old: list Z, d:val, 
+       data: val, dsh:share, new: list Z, len:int
+  PRE [ 1%positive OF (tptr (Tstruct _env_md_ctx_st noattr)), 
+        2%positive OF tptr tvoid, 3%positive OF tuint]
+       PROP (readable_share dsh)
+       LOCAL (temp 1%positive ctx; temp 2%positive data; temp 3%positive (Vint len) )
+       SEP (MDCTXHashed nid ctxsz old d ctx;
+            data_at dsh (tarray tuchar (Int.unsigned len)) (map Vint (map Int.repr new)) data)
+  POST [ tvoid ]
+          PROP() LOCAL () 
+          SEP(MDCTXHashed nid ctxsz (old++new) d ctx;
+              data_at dsh (tarray tuchar (Int.unsigned len)) (map Vint (map Int.repr new)) data).
+
+Definition EVP_DigestUpdate_SPEC := DECLARE _EVP_DigestUpdate
+  WITH ctx: val, nid:int, ctxsz:int, old: list Z, d:val, 
+       data: val, dsh:share, new: list Z, len:int, 
+       tsh:share, vals:reptype (Tstruct _env_md_st noattr)
+  PRE [ _ctx OF tptr (Tstruct _env_md_ctx_st noattr), _data OF tptr tvoid,  _len OF tuint ]
+      PROP (readable_share dsh; readable_share tsh)
+      LOCAL (temp _ctx ctx; temp _data data; temp _len (Vint len) )
+      SEP (MDCTXHashed nid ctxsz old d ctx;
+            data_at dsh (tarray tuchar (Int.unsigned len)) (map Vint (map Int.repr new)) data;
+            EVP_MD_NNnode tsh vals d;
+            func_ptr' upd_spec (get_updptr vals))
+  POST [ tint] 
+       PROP ()
+       LOCAL (temp ret_temp (Vint Int.one))
+       SEP (MDCTXHashed nid ctxsz (old++new) d ctx;
+            data_at dsh (tarray tuchar (Int.unsigned len)) (map Vint (map Int.repr new)) data;
+              EVP_MD_NNnode tsh vals d;
+              func_ptr' upd_spec (get_updptr vals)).
+
+Definition Gprog_DigestUpdate : funspecs :=
+  (*FAILS TO TERMINATE: ltac:(with_library prog [EVP_MD_type_SPEC]). *)
+  [].
+
+Axiom body_DigestUpdate: semax_body Vprog Gprog_DigestUpdate f_EVP_DigestUpdate EVP_DigestUpdate_SPEC.
+
+Definition fin_spec:funspec :=
+  WITH ctx: val, nid:int, ctxsz:int, content: list Z, d:val,
+       out: val, osh:share, len:Z
+  PRE [ 1%positive OF tptr (Tstruct _env_md_ctx_st noattr),
+        2%positive OF tptr tuchar]
+       PROP (writable_share osh)
+       LOCAL (temp 1%positive ctx; temp 2%positive out)
+       SEP (MDCTXHashed nid ctxsz content d ctx; 
+            memory_block osh len out)
+  POST [ tvoid ]
+          PROP() LOCAL () 
+          SEP(MDCTXFinished nid ctxsz d ctx;
+              data_at osh (tarray tuchar len) (map Vint (map Int.repr content)) out).
+
+Definition EVP_DigestFinal_ex_SPEC := DECLARE _EVP_DigestFinal_ex
+  WITH ctx: val, nid:int, ctxsz:int, content: list Z, d:val,
+       out: val, osh:share, sz:val, tsh:share,
+       vals:reptype (Tstruct _env_md_st noattr), mdsize:int
+  PRE [ _ctx OF tptr (Tstruct _env_md_ctx_st noattr),
+        _md_out OF tptr tuchar, _size OF tptr tuint]
+      PROP (writable_share osh; readable_share tsh;
+            get_mdsize vals = Vint mdsize;
+            get_ctxsize vals = Vint ctxsz; 0 <= Int.unsigned ctxsz <= Int.max_unsigned)
+      LOCAL (temp _ctx ctx; temp _md_out out; temp _size sz)
+      SEP (MDCTXHashed nid ctxsz content d ctx; 
+            memory_block osh (Int.unsigned mdsize) out;
+            EVP_MD_NNnode tsh vals d;
+            func_ptr' fin_spec (get_finptr vals); 
+            if Val.eq sz nullval then emp else data_at_ Tsh tuint sz)
+  POST [ tint] 
+       PROP ()
+       LOCAL (temp ret_temp (Vint Int.one))
+       SEP (MDCTXFinished nid ctxsz d ctx;
+              data_at osh (tarray tuchar (Int.unsigned mdsize)) (map Vint (map Int.repr content)) out;
+              EVP_MD_NNnode tsh vals d;
+              func_ptr' fin_spec (get_finptr vals);
+              if Val.eq sz nullval then emp else data_at Tsh tuint (Vint mdsize) sz).
+
+Definition Gprog_DigestFinal_ex : funspecs :=
+  (*FAILS TO TERMINATE: ltac:(with_library prog [EVP_MD_type_SPEC]). *)
+  [OPENSSL_cleanse_SPEC].
+
+Axiom body_DigestFinal_ex: semax_body Vprog Gprog_DigestFinal_ex f_EVP_DigestFinal_ex EVP_DigestFinal_ex_SPEC.
+
+Definition EVP_DigestFinal_SPEC := DECLARE _EVP_DigestFinal
+  WITH ctx: val, nid:int, ctxsz:int, content: list Z, d:val,
+       out: val, osh:share, sz:val, tsh:share,
+       vals:reptype (Tstruct _env_md_st noattr), mdsize:int
+  PRE [ _ctx OF tptr (Tstruct _env_md_ctx_st noattr),
+        _md OF tptr tuchar, _size OF tptr tuint]
+      PROP (writable_share osh; readable_share tsh;
+            get_mdsize vals = Vint mdsize;
+            get_ctxsize vals = Vint ctxsz; 0 <= Int.unsigned ctxsz <= Int.max_unsigned;
+            get_type vals = Vint nid)
+      LOCAL (temp _ctx ctx; temp _md out; temp _size sz)
+      SEP (MDCTXHashed nid ctxsz content d ctx; 
+            memory_block osh (Int.unsigned mdsize) out;
+            EVP_MD_NNnode tsh vals d;
+            func_ptr' fin_spec (get_finptr vals); 
+            if Val.eq sz nullval then emp else data_at_ Tsh tuint sz)
+  POST [ tint] 
+       PROP ()
+       LOCAL (temp ret_temp (Vint Int.one))
+       SEP (MDCTXInitialized ctx; EVP_MD_NNnode tsh vals d;
+            data_at osh (tarray tuchar (Int.unsigned mdsize)) (map Vint (map Int.repr content)) out;
+            func_ptr' fin_spec (get_finptr vals);
+            if Val.eq sz nullval then emp else data_at Tsh tuint (Vint mdsize) sz).
+
+Definition Gprog_DigestFinal : funspecs :=
+  (*FAILS TO TERMINATE: ltac:(with_library prog [EVP_MD_type_SPEC]). *)
+  [EVP_DigestFinal_ex_SPEC; EVP_MD_CTX_cleanup_SPEC].
+
+Axiom body_DigestFinal: semax_body Vprog Gprog_DigestFinal f_EVP_DigestFinal EVP_DigestFinal_SPEC.
+
+
+(*Adam2: State MDCTXAllocated ictx must be ruled out, ie if ictx is nonnull, 
+  it must also be initialized already. Otherwise the access to 
+  in -> digest in the first conditional will access a Vundef.
+  (Alternative: we change the def of Allocated...)*)
+
+Definition Gprog_copy_ex : funspecs :=
+  (*FAILS TO TERMINATE: ltac:(with_library prog [EVP_MD_type_SPEC]). *)
+  [EVP_MD_CTX_cleanup_SPEC; OPENSSL_PUT_ERROR_SPEC; OPENSSL_malloc_SPEC; OPENSSL_memcpy_STRONGSPEC ].
+(*note use of strongspec here! Without it, we'd have to prove a lemma like the following (and maybe its inverse)
+  (Of course, such a lemma may be needed to justify memcpy strongspec...
+Lemma DigestRep_changeREP tp v data md
+  (D: DigestRep tp v (map Int.unsigned data)):
+  data_at Tsh tp v md = data_at Tsh (tarray tuchar (sizeof tp)) (map Vint data) md.
+Admitted.*)
+
+Inductive EVP_MD_CTX_copy_case :=
+  CopyInitialized: EVP_MD_CTX_copy_case
+| CopyHashedFinished: forall (dsh:share) (vals:reptype (Tstruct _env_md_st noattr))
+                             (data: option (list int)) (d:val), EVP_MD_CTX_copy_case.
+
+Definition EVP_MD_CTX_copy_pre (c:EVP_MD_CTX_copy_case) (octx ictx:val) : mpred :=
+  match c with
+   CopyInitialized => MDCTXInitialized ictx
+ | CopyHashedFinished dsh vals data d => 
+     EX nid:int, EX ctxsz:int, 
+     !!(get_ctxsize vals = Vint ctxsz /\ 4 <= Int.unsigned ctxsz <= Int.max_unsigned)
+     && match data with None => MDCTXFinished nid ctxsz d ictx
+                     | Some v => MDCTXHashed nid ctxsz (map Int.unsigned v) d ictx
+        end * 
+        EVP_MD_NNnode dsh vals d * MDCTXInitialized octx
+ end.
+
+Definition EVP_MD_CTX_copy_post (c:EVP_MD_CTX_copy_case) (octx ictx rv:val) : mpred :=
+  match c with
+   CopyInitialized => !!(rv=nullval)&& MDCTXInitialized ictx
+ | CopyHashedFinished dsh vals data d => 
+     EX nid:int, EX ctxsz:int, 
+     !!(get_ctxsize vals = Vint ctxsz /\ 4 <= Int.unsigned ctxsz <= Int.max_unsigned)
+     && match data with None => MDCTXFinished nid ctxsz d ictx
+                     | Some v => MDCTXHashed nid ctxsz (map Int.unsigned v) d ictx
+        end * EVP_MD_NNnode dsh vals d *
+        ( (!!(rv=nullval) && MDCTXInitializedDigestSet d octx)
+          || (!!(rv=Vone) && match data with None => MDCTXFinished nid ctxsz d octx
+                                           | Some v => MDCTXHashed nid ctxsz (map Int.unsigned v) d octx
+                             end ))
+ end.
+
+Definition EVP_MD_CTX_copy_ex_SPEC := DECLARE _EVP_MD_CTX_copy_ex
+  WITH ep: val, octx:val, ictx:val, c: EVP_MD_CTX_copy_case
+  PRE [ _out OF (tptr (Tstruct _env_md_ctx_st noattr)),
+        _in OF (tptr (Tstruct _env_md_ctx_st noattr)) ]
+      PROP ()
+      LOCAL (gvar ___stringlit_1 ep; temp _out octx; temp _in ictx)
+      SEP (ERR ep; EVP_MD_CTX_copy_pre c octx ictx)
+  POST [ tint] EX rv:val,
+       PROP ()
+       LOCAL (temp ret_temp rv)
+       SEP (ERR ep; EVP_MD_CTX_copy_post c octx ictx rv).
+
+Axiom body_EVP_MD_CTX_copy_ex: semax_body Vprog Gprog_copy_ex f_EVP_MD_CTX_copy_ex EVP_MD_CTX_copy_ex_SPEC.
+
+(*Also supports Hashed octx, since Hashed octx |-- Finished octx. (BUT THAT'S NOT EXPOSED!
+  Allocation is performed, and result may be Vone or Vnull*)
+Definition EVP_MD_CTX_copy_ex_SPEC_Finished_NEQ := DECLARE _EVP_MD_CTX_copy_ex
+  WITH ep: val, octx:val, ictx:val,
+       nid:int, ctxsz:int, sh:share * share, vals:_, t:val,
+       nid':int, ctxsz':int, d:val
+  PRE [ _out OF (tptr (Tstruct _env_md_ctx_st noattr)),
+        _in OF (tptr (Tstruct _env_md_ctx_st noattr)) ]
+      PROP (get_ctxsize (snd vals) = Vint ctxsz' /\ get_type (snd vals) = Vint nid';
+            get_ctxsize (fst vals) = Vint ctxsz; 4 <= Int.unsigned ctxsz <= Int.max_unsigned; d<>t)
+      LOCAL (gvar ___stringlit_1 ep; temp _out octx; temp _in ictx)
+      SEP (ERR ep; MDCTXFinished nid' ctxsz' d octx; 
+           MDCTXFinished nid ctxsz t ictx;
+           EVP_MD_NNnode (fst sh) (fst vals) t; EVP_MD_NNnode (snd sh) (snd vals) d)
+  POST [ tint] EX rv:_,
+       PROP ()
+       LOCAL (temp ret_temp rv)
+       SEP (ERR ep; MDCTXFinished nid ctxsz t ictx; 
+            EVP_MD_NNnode (fst sh) (fst vals) t; EVP_MD_NNnode (snd sh) (snd vals) d;
+            (!!(rv=nullval) && MDCTXInitializedDigestSet t octx) 
+            || (!!(rv=Vone) && MDCTXFinished nid ctxsz t octx)).
+
+(*Also supports Hashed octx, since Hashed octx |-- Finished octx.
+  No allocation is performed, and result value is always Vone*)
+Definition EVP_MD_CTX_copy_ex_SPEC_Finished_EQ := DECLARE _EVP_MD_CTX_copy_ex
+  WITH ep: val, octx:val, ictx:val,
+       nid:int, ctxsz:int, tsh:share, vals:_, t:val
+  PRE [ _out OF (tptr (Tstruct _env_md_ctx_st noattr)),
+        _in OF (tptr (Tstruct _env_md_ctx_st noattr)) ]
+      PROP (get_ctxsize vals = Vint ctxsz; 4 <= Int.unsigned ctxsz <= Int.max_unsigned)
+      LOCAL (gvar ___stringlit_1 ep; temp _out octx; temp _in ictx)
+      SEP (ERR ep; MDCTXFinished nid ctxsz t octx; 
+           MDCTXFinished nid ctxsz t ictx;
+           EVP_MD_NNnode tsh vals t)
+  POST [ tint] 
+       PROP ()
+       LOCAL (temp ret_temp Vone)
+       SEP (ERR ep; MDCTXFinished nid ctxsz t ictx; EVP_MD_NNnode tsh vals t;
+            MDCTXFinished nid ctxsz t octx).
+
+Axiom body_EVP_MD_CTX_copy_ex_Finished_NEQ: semax_body Vprog Gprog_copy_ex f_EVP_MD_CTX_copy_ex EVP_MD_CTX_copy_ex_SPEC_Finished_NEQ.
+
+Axiom body_EVP_MD_CTX_copy_ex_FinishedEQ: semax_body Vprog Gprog_copy_ex f_EVP_MD_CTX_copy_ex EVP_MD_CTX_copy_ex_SPEC_Finished_EQ.
+
+(*Also supports Hashed octx, since Hashed octx |-- Finished octx.
+  Allocation is performed, and result may be Vone or Vnull*)
+Definition EVP_MD_CTX_copy_ex_SPEC_Hashed_NEQ := DECLARE _EVP_MD_CTX_copy_ex
+  WITH ep: val, octx:val, ictx:val,
+       nid:int, ctxsz:int , data:list int, sh:share * share, vals:_, t:val,
+       nid':int, ctxsz':int, d:val
+  PRE [ _out OF (tptr (Tstruct _env_md_ctx_st noattr)),
+        _in OF (tptr (Tstruct _env_md_ctx_st noattr)) ]
+      PROP (get_ctxsize (snd vals) = Vint ctxsz' /\ get_type (snd vals) = Vint nid';
+            get_ctxsize (fst vals) = Vint ctxsz; 4 <= Int.unsigned ctxsz <= Int.max_unsigned; d<>t)
+      LOCAL (gvar ___stringlit_1 ep; temp _out octx; temp _in ictx)
+      SEP (ERR ep; MDCTXFinished nid' ctxsz' d octx; 
+           MDCTXHashed nid ctxsz (map Int.unsigned data) t ictx;
+           EVP_MD_NNnode (fst sh) (fst vals) t; EVP_MD_NNnode (snd sh) (snd vals) d)
+  POST [ tint] EX rv:_,
+       PROP ()
+       LOCAL (temp ret_temp rv)
+       SEP (ERR ep; MDCTXHashed nid ctxsz (map Int.unsigned data) t ictx; 
+            EVP_MD_NNnode (fst sh) (fst vals) t; EVP_MD_NNnode (snd sh) (snd vals) d;
+            (!!(rv=nullval) && MDCTXInitializedDigestSet t octx) 
+            || (!!(rv=Vone) && MDCTXHashed nid ctxsz (map Int.unsigned data) t octx)).
+
+(*Also supports Hashed octx, since Hashed octx |-- Finished octx.
+  No allocation is performed, and result value is always Vone*)
+Definition EVP_MD_CTX_copy_ex_SPEC_Hashed_EQ := DECLARE _EVP_MD_CTX_copy_ex
+  WITH ep: val, octx:val, ictx:val,
+       nid:int, ctxsz:int, data:list int, tsh:share, vals:_, t:val
+  PRE [ _out OF (tptr (Tstruct _env_md_ctx_st noattr)),
+        _in OF (tptr (Tstruct _env_md_ctx_st noattr)) ]
+      PROP (get_ctxsize vals = Vint ctxsz; 4 <= Int.unsigned ctxsz <= Int.max_unsigned)
+      LOCAL (gvar ___stringlit_1 ep; temp _out octx; temp _in ictx)
+      SEP (ERR ep; MDCTXFinished nid ctxsz t octx; 
+           MDCTXHashed nid ctxsz (map Int.unsigned data) t ictx;
+           EVP_MD_NNnode tsh vals t)
+  POST [ tint] 
+       PROP ()
+       LOCAL (temp ret_temp Vone)
+       SEP (ERR ep; MDCTXHashed nid ctxsz (map Int.unsigned data) t ictx; EVP_MD_NNnode tsh vals t;
+            MDCTXHashed nid ctxsz (map Int.unsigned data) t octx).
+
+
+Axiom body_EVP_MD_CTX_copy_ex_Hashed_NEQ: semax_body Vprog Gprog_copy_ex f_EVP_MD_CTX_copy_ex EVP_MD_CTX_copy_ex_SPEC_Hashed_NEQ.
+
+Axiom body_EVP_MD_CTX_copy_ex_HashedEQ: semax_body Vprog Gprog_copy_ex f_EVP_MD_CTX_copy_ex EVP_MD_CTX_copy_ex_SPEC_Hashed_EQ.
+
+End EVP_MD_CTX_Protocol_TP.
+
+Module EVP_MD_CTX_Protocol <: EVP_MD_CTX_Protocol_TP.
+
 Definition MDCTXInitialized p : mpred := 
   data_at Tsh (Tstruct _env_md_ctx_st noattr) (nullval, (nullval, (nullval, nullval))) p.
 
 Definition MDCTXAllocated p : mpred := 
   data_at_ Tsh (Tstruct _env_md_ctx_st noattr) p.
+
+(*Propose to Adam that this be eliminated - it's needed in 3 places*)
+Definition MDCTXInitializedDigestSet t p : mpred := 
+  !!(isptr t) && data_at Tsh (Tstruct _env_md_ctx_st noattr) (t, (nullval, (nullval, nullval))) p.
 
 Lemma MDCTXAllocated_valid_ptr p: MDCTXAllocated p |-- valid_pointer p.
 Proof. unfold MDCTXAllocated. apply data_at_valid_ptr; [ intuition | simpl; omega]. Qed.
@@ -493,8 +1196,14 @@ Proof. unfold MDCTXAllocated. apply data_at_valid_ptr; [ intuition | simpl; omeg
 Lemma MDCTXInitialized_MDCTXAllocated p: MDCTXInitialized p|-- MDCTXAllocated p.
 Proof. unfold MDCTXInitialized, MDCTXAllocated; cancel. Qed.
 
+Lemma MDCTXInitializedDigestSet_MDCTXAllocated t p: MDCTXInitializedDigestSet t p|-- MDCTXAllocated p.
+Proof. unfold MDCTXInitializedDigestSet, MDCTXAllocated. entailer!. Qed.
+
 Lemma MDCTXInitialized_valid_ptr p: MDCTXInitialized p |-- valid_pointer p.
 Proof. eapply derives_trans; [ apply MDCTXInitialized_MDCTXAllocated | apply MDCTXAllocated_valid_ptr]. Qed.
+
+Lemma MDCTXInitializedDigestSet_valid_ptr t p: MDCTXInitializedDigestSet t p |-- valid_pointer p.
+Proof. eapply derives_trans; [ apply MDCTXInitializedDigestSet_MDCTXAllocated | apply MDCTXAllocated_valid_ptr]. Qed.
 
 Lemma MDCTXAllocated_isptr p: MDCTXAllocated p |-- !! isptr p.
 Proof. unfold MDCTXAllocated; entailer!. Qed.
@@ -502,22 +1211,24 @@ Proof. unfold MDCTXAllocated; entailer!. Qed.
 Lemma MDCTXInitialized_isptr p: MDCTXInitialized p |-- !! isptr p.
 Proof. eapply derives_trans; [ apply MDCTXInitialized_MDCTXAllocated | apply MDCTXAllocated_isptr]. Qed.
 
+Lemma MDCTXInitializedDigestSet_isptr t p: MDCTXInitializedDigestSet t p |-- !! isptr p.
+Proof. eapply derives_trans; [ apply MDCTXInitializedDigestSet_MDCTXAllocated | apply MDCTXAllocated_isptr]. Qed.
+
 Lemma MDCTXAllocated_isptr' p: MDCTXAllocated p = (!!isptr p) && MDCTXAllocated p.
 Proof. apply pred_ext; entailer; apply MDCTXAllocated_isptr. Qed.
 
 Lemma MDCTXInitialized_isptr' p: MDCTXInitialized p = (!! isptr p) && MDCTXInitialized p.
 Proof. apply pred_ext; entailer; apply MDCTXInitialized_isptr. Qed.
 
+Lemma MDCTXInitializedDigestSet_isptr' t p: MDCTXInitializedDigestSet t p = (!! isptr p) && MDCTXInitializedDigestSet t p.
+Proof. apply pred_ext; entailer; apply MDCTXInitializedDigestSet_isptr. Qed.
+
 Definition EVP_MD_CTX_init_SPEC := DECLARE _EVP_MD_CTX_init
    WITH ctx:val
    PRE [ _ctx OF tptr (Tstruct _env_md_ctx_st noattr) ]
-       PROP ()
-       LOCAL (temp _ctx ctx)
-       SEP (MDCTXAllocated ctx)
+       PROP () LOCAL (temp _ctx ctx) SEP (MDCTXAllocated ctx)
    POST [ tvoid ]
-       PROP ()
-       LOCAL ()
-       SEP (MDCTXInitialized ctx).
+       PROP () LOCAL () SEP (MDCTXInitialized ctx).
 
 Definition EVP_MD_CTX_create_SPEC := DECLARE _EVP_MD_CTX_create
    WITH ctx:val
@@ -562,36 +1273,6 @@ Proof.
   - subst; contradiction. 
   - forward. Exists v; entailer!. apply orp_right2; trivial. 
 Qed.
-
-
-(****** Specs of the four Digest Operation Accessors. *******)
-(*nonnull node*)
-Definition EVP_MD_CTX_NNnode (sh:share) (vals:val*(val*(val*val))) (p:val):mpred :=
-  match vals with (d, (mddata, (pctx, pctxops))) =>
-  !!(is_pointer_or_null d /\ is_pointer_or_null mddata) &&
-  data_at sh (Tstruct _env_md_ctx_st noattr) (d,(mddata,(pctx, pctxops))) p
-  end.
-
-Lemma EVP_MD_CTX_NNnode_isptr sh vals p:
-  EVP_MD_CTX_NNnode sh vals p |-- !!(isptr p).
-Proof.
-  unfold EVP_MD_CTX_NNnode. destruct vals as [d [mdd [pc pcops]]]. normalize.
-  rewrite data_at_isptr. entailer!.
-Qed.
-Lemma EVP_MD_CTX_NNnode_isptr' sh vals p:
-  EVP_MD_CTX_NNnode sh vals p  = (!!(isptr p) &&  EVP_MD_CTX_NNnode sh vals p).
-Proof.
-  apply pred_ext; [ entailer; apply EVP_MD_CTX_NNnode_isptr | entailer!].
-Qed.
-
-(*a possibly null node*)
-Definition EVP_MD_CTX_node sh (vals:val*(val*(val*val))) (p:val):mpred :=
- (!!(p = nullval) && emp) || EVP_MD_CTX_NNnode sh vals p.
-
-Lemma EVP_MD_CTX_node_null sh vals: EVP_MD_CTX_node sh vals nullval |-- emp.
-Proof. apply orp_left; [| rewrite EVP_MD_CTX_NNnode_isptr']; normalize. Qed.
-
-Hint Resolve EVP_MD_CTX_node_null: cancel.
 
 (*According to digest.h, EVP_MD_CTX_md may be invoked even if no digest has not been set, 
   returning null in this case. The other 3 functions are specified to crash in such a 
@@ -701,105 +1382,24 @@ Proof.
   normalize. apply orp_right2. unfold EVP_MD_CTX_NNnode. entailer!.
 Qed.  
 
-(*nonnull node*)
-Definition EVP_MD_NNnode (sh:share) (vals:reptype (Tstruct _env_md_st noattr)) (p:val):mpred :=
-  !!(readable_share sh) &&
-  data_at sh (Tstruct _env_md_st noattr) vals p.
-
-Lemma EVP_MD_NNnode_isptr sh vals p:
-  EVP_MD_NNnode sh vals p |-- !!(isptr p).
-Proof.
-  unfold EVP_MD_NNnode. destruct vals. normalize.
-  rewrite data_at_isptr. entailer!.
-Qed.
-Lemma EVP_MD_NNnode_isptr' sh vals p:
-  EVP_MD_NNnode sh vals p  = (!!(isptr p) &&  EVP_MD_NNnode sh vals p).
-Proof.
-  apply pred_ext; [ entailer; apply EVP_MD_NNnode_isptr | entailer!].
-Qed.
-
-Lemma EVP_MD_NNnode_validptr sh vals p:  EVP_MD_NNnode sh vals p |-- valid_pointer p.
-Proof. unfold EVP_MD_NNnode. entailer!. Qed.
-
-(*a possibly null node*)
-Definition EVP_MD_node (vals:reptype (Tstruct _env_md_st noattr))(p:val):mpred :=
- (!!(p = nullval) && emp) || (EX sh:_, EVP_MD_NNnode sh vals p).
-
-
-Lemma EVP_MD_node_null vals: EVP_MD_node vals nullval |-- emp.
-Proof. apply orp_left; [| Intros sh; rewrite EVP_MD_NNnode_isptr' ]; normalize. Qed.
-
-Hint Resolve EVP_MD_node_null: cancel.
-
-Lemma EVP_MD_node_validptr vals p:  EVP_MD_node vals p |-- valid_pointer p.
-Proof. unfold EVP_MD_node.
-  apply orp_left; normalize. apply valid_pointer_null.
-  apply EVP_MD_NNnode_validptr. 
-Qed.
-
-Definition get_type (vals:reptype (Tstruct _env_md_st noattr)):=
-  match vals with
-    (type, (mds, (flags, (ini, (upd, (fin, (blsize, ctxsize))))))) => type
-  end.
-Definition get_mdsize (vals:reptype (Tstruct _env_md_st noattr)):=
-  match vals with
-    (type, (mds, (flags, (ini, (upd, (fin, (blsize, ctxsize))))))) => mds
-  end.
-Definition get_iniptr (vals:reptype (Tstruct _env_md_st noattr)):=
-  match vals with
-    (type, (mds, (flags, (ini, (upd, (fin, (blsize, ctxsize))))))) => ini
-  end.
-Definition get_updptr (vals:reptype (Tstruct _env_md_st noattr)):=
-  match vals with
-    (type, (mds, (flags, (ini, (upd, (fin, (blsize, ctxsize))))))) => upd
-  end.
-Definition get_finptr (vals:reptype (Tstruct _env_md_st noattr)):=
-  match vals with
-    (type, (mds, (flags, (ini, (upd, (fin, (blsize, ctxsize))))))) => fin
-  end.
-Definition get_blsize (vals:reptype (Tstruct _env_md_st noattr)):=
-  match vals with
-    (type, (mds, (flags, (ini, (upd, (fin, (blsize, ctxsize))))))) => blsize
-  end.
-Definition get_ctxsize (vals:reptype (Tstruct _env_md_st noattr)):=
-  match vals with
-    (type, (mds, (flags, (ini, (upd, (fin, (blsize, ctxsize))))))) => ctxsize
-  end.
-
-Lemma Valeq_Vint {A} i j (a b:A):
-      (if Val.eq (Vint i) (Vint j) then a else b) =
-      (if Int.eq i j then a else b).
-Proof. 
- remember (Int.eq i j). destruct b0.
-+ rewrite ( binop_lemmas2.int_eq_true _ _ Heqb0). rewrite if_true; trivial.
-+ remember (Val.eq (Vint i )(Vint j)) as d.
-  destruct d; trivial.
-  inversion e; subst; simpl in *.
-  specialize (int_eq_false_e j j); intuition.
-Qed. 
-
 Definition Gprog_cleanup : funspecs :=
   (*FAILS TO TERMINATE: ltac:(with_library prog [EVP_MD_type_SPEC]). *)
   [OPENSSL_cleanse_SPEC; OPENSSL_free_SPEC; EVP_MD_CTX_init_SPEC].
 
 Parameter struct_of_nid: int -> option type.
+Parameter DigestRep: forall (t:type) (v:reptype t) (data:list Z), Prop. (*should generalize s256_relate*)
+Parameter DigestRepNil: forall t, DigestRep t (default_val t) [].
+
 Definition postInit (nid:int) (ctxsz:Z) (p:val):mpred :=
   EX t:type, !!(struct_of_nid nid = Some t /\ sizeof t = ctxsz)
      && data_at_ Tsh t p.
 Lemma postInit_memblock nid ctxsz m:
   postInit nid (Int.unsigned ctxsz) m |-- memory_block Tsh (Int.unsigned ctxsz) m.
 Proof. unfold postInit; Intros t. rewrite data_at__memory_block, H0; entailer!. Qed.
-(*
-Definition MDCTXConfigured ctxsz (d p:val): mpred :=
-  EX md:val, !!(Int.eq ctxsz Int.zero=false) && EVP_MD_CTX_NNnode Tsh (d,(md,(nullval,nullval))) p *
-             memory_block Tsh (Int.unsigned ctxsz) md.*)
 
 Definition MDCTXConfigured nid ctxsz (d p:val): mpred :=
   EX md:val, !!(Int.eq ctxsz Int.zero=false) && EVP_MD_CTX_NNnode Tsh (d,(md,(nullval,nullval))) p *
              postInit nid (Int.unsigned ctxsz) md.
-
-Parameter DigestRep: forall (t:type) (v:reptype t) (data:list Z), Prop. (*should generalize s256_relate*)
-Parameter DigestRepNil: forall t, DigestRep t (default_val t) [].
 
 Definition MDCTXHashed nid ctxsz (data:list Z) (d p:val): mpred :=
   EX md:val, EX t:type, EX v: reptype t,
@@ -813,34 +1413,6 @@ Definition MDCTXFinished nid ctxsz (d p:val): mpred :=
        !!(Int.eq ctxsz Int.zero=false /\ struct_of_nid nid = Some t /\ sizeof t = Int.unsigned ctxsz)
        && EVP_MD_CTX_NNnode Tsh (d,(md,(nullval,nullval))) p *
              data_at_ Tsh t md.
-
-Inductive EVP_MD_CTX_cleanup_case :=
-  ClInitialized: EVP_MD_CTX_cleanup_case
-| ClConfiguredOrFinished: forall (dsh:share) (vals:reptype (Tstruct _env_md_st noattr)) (d:val), EVP_MD_CTX_cleanup_case.
-
-Definition EVP_MD_CTX_cleanup_pre (c:EVP_MD_CTX_cleanup_case) (ctx:val) : mpred :=
-  match c with
-   ClInitialized => MDCTXInitialized ctx
- | ClConfiguredOrFinished dsh vals d => 
-     EX nid:int, EX ctxsz:int, 
-     !!(get_ctxsize vals = Vint ctxsz /\ get_type vals = Vint nid)
-     && (MDCTXConfigured nid ctxsz d ctx || MDCTXFinished nid ctxsz d ctx) * EVP_MD_NNnode dsh vals d
-end.
-
-Definition EVP_MD_CTX_cleanup_post (c:EVP_MD_CTX_cleanup_case) (ctx:val) : mpred :=
-  match c with
-   ClInitialized => MDCTXInitialized ctx
- | ClConfiguredOrFinished dsh vals d => MDCTXInitialized ctx * EVP_MD_NNnode dsh vals d
-end.
-
-Definition EVP_MD_CTX_cleanup_SPEC := DECLARE _EVP_MD_CTX_cleanup
-  WITH ctx:val, c:EVP_MD_CTX_cleanup_case
-  PRE [ _ctx OF (tptr (Tstruct _env_md_ctx_st noattr)) ]
-      PROP () LOCAL (temp _ctx ctx)
-      SEP (EVP_MD_CTX_cleanup_pre c ctx)
-  POST [ tint ]
-       PROP () LOCAL (temp ret_temp (Vint (Int.one)))
-       SEP (EVP_MD_CTX_cleanup_post c ctx).
 
 Lemma MDCTXConfigured_valid_ptr nid ctxsz d p: MDCTXConfigured nid ctxsz d p |-- valid_pointer p.
 Proof. unfold MDCTXConfigured, EVP_MD_CTX_NNnode; entailer. Qed.
@@ -874,7 +1446,7 @@ Lemma MDCTXFinished_MDCTXConfigured nid ctxsz d p: MDCTXFinished nid ctxsz d p =
 Proof. unfold MDCTXFinished, MDCTXConfigured, postInit; apply pred_ext; Intros md t; Exists md t; entailer!. Qed.
 
 (*This lemma is not to be exposed!*)
-Lemma MDCTXHashed_MDCTX_Finished nid ctxsz data d p: MDCTXHashed nid ctxsz data d p |-- MDCTXFinished nid ctxsz d p.
+Lemma MDCTXHashed_MDCTXFinished nid ctxsz data d p: MDCTXHashed nid ctxsz data d p |-- MDCTXFinished nid ctxsz d p.
 Proof. unfold MDCTXFinished, MDCTXHashed; Intros md t v. Exists md t; entailer!. Qed.
 
 Lemma MDCTXFinished_valid_ptr nid ctxsz d p: MDCTXFinished nid ctxsz d p |-- valid_pointer p.
@@ -886,6 +1458,64 @@ Proof. rewrite MDCTXFinished_MDCTXConfigured. apply MDCTXConfigured_isptr. Qed.
 Lemma MDCTXFinished_isptr' nid ctxsz d p:
       MDCTXFinished nid ctxsz d p = (!!isptr p) && MDCTXFinished nid ctxsz d p.
 Proof. apply pred_ext; entailer; apply MDCTXFinished_isptr. Qed.
+
+Definition MDCTXHashedOrFinished nid ctxsz d p: mpred :=
+  (EX data:_, MDCTXHashed nid ctxsz (map Int.unsigned data) d p)
+  || MDCTXFinished nid ctxsz d p.
+
+Lemma MDCTXHashedOrFinished_valid_ptr nid ctxsz d p: 
+      MDCTXHashedOrFinished nid ctxsz d p |-- valid_pointer p.
+Proof. apply orp_left; [ Intros data; apply MDCTXHashed_valid_ptr | apply MDCTXFinished_valid_ptr ]. Qed.
+ 
+Lemma MDCTXHashedOrFinished_isptr nid ctxsz d p: 
+  MDCTXHashedOrFinished nid ctxsz d p |-- !!(isptr p).
+Proof.
+  apply orp_left; [ Intros data; apply MDCTXHashed_isptr | apply MDCTXFinished_isptr ]. 
+Qed.
+Lemma MDCTXHashedOrFinished_isptr' nid ctxsz d p: 
+  MDCTXHashedOrFinished nid ctxsz d p = !!(isptr p) && MDCTXHashedOrFinished nid ctxsz d p.
+Proof. apply pred_ext; entailer; apply MDCTXHashedOrFinished_isptr. Qed.
+
+(*This lemma is not exposed*)
+Lemma MDCTXHashedOrFinished_MDCTXFinished nid ctxsz d p: 
+  MDCTXHashedOrFinished nid ctxsz d p = MDCTXFinished nid ctxsz d p.
+Proof. apply pred_ext.
+  apply orp_left; [ Intros data; apply MDCTXHashed_MDCTXFinished | trivial].
+  apply orp_right2; trivial.
+Qed.
+
+Inductive EVP_MD_CTX_cleanup_case :=
+  ClInitialized: EVP_MD_CTX_cleanup_case
+| ClInitializedDigestSet: forall (d:val) (dsh:share) (vals:reptype (Tstruct _env_md_st noattr)), EVP_MD_CTX_cleanup_case (*Talk with Adam to allow removal of this*)
+| ClConfiguredOrFinished: forall (dsh:share) (vals:reptype (Tstruct _env_md_st noattr)) (d:val), EVP_MD_CTX_cleanup_case.
+
+Definition EVP_MD_CTX_cleanup_pre (c:EVP_MD_CTX_cleanup_case) (ctx:val) : mpred :=
+  match c with
+   ClInitialized => MDCTXInitialized ctx
+ | ClInitializedDigestSet t tsh vals => EX ctxsz:int, 
+     !!(get_ctxsize vals = Vint ctxsz /\ Int.eq ctxsz Int.zero = false)
+     && MDCTXInitializedDigestSet t ctx * EVP_MD_NNnode tsh vals t
+ | ClConfiguredOrFinished dsh vals d => 
+     EX nid:int, EX ctxsz:int, 
+     !!(get_ctxsize vals = Vint ctxsz /\ get_type vals = Vint nid)
+     && (MDCTXConfigured nid ctxsz d ctx || MDCTXFinished nid ctxsz d ctx) * EVP_MD_NNnode dsh vals d
+end.
+
+Definition EVP_MD_CTX_cleanup_post (c:EVP_MD_CTX_cleanup_case) (ctx:val) : mpred :=
+  match c with
+   ClInitialized => MDCTXInitialized ctx
+ | ClInitializedDigestSet t tsh vals => MDCTXInitialized ctx * EVP_MD_NNnode tsh vals t
+ | ClConfiguredOrFinished dsh vals d => MDCTXInitialized ctx * EVP_MD_NNnode dsh vals d
+end.
+
+Definition EVP_MD_CTX_cleanup_SPEC := DECLARE _EVP_MD_CTX_cleanup
+  WITH ctx:val, c:EVP_MD_CTX_cleanup_case
+  PRE [ _ctx OF (tptr (Tstruct _env_md_ctx_st noattr)) ]
+      PROP () LOCAL (temp _ctx ctx)
+      SEP (EVP_MD_CTX_cleanup_pre c ctx)
+  POST [ tint ]
+       PROP () LOCAL (temp ret_temp (Vint (Int.one)))
+       SEP (EVP_MD_CTX_cleanup_post c ctx).
 
 Lemma body_EVP_MD_CTX_cleanup: semax_body Vprog Gprog_cleanup f_EVP_MD_CTX_cleanup EVP_MD_CTX_cleanup_SPEC.
 Proof. 
@@ -915,6 +1545,42 @@ Proof.
     [ inv H | clear H; forward; entailer! | ].
   forward_call (ctx). { unfold MDCTXAllocated. cancel. }
   forward.
++ (*InitializedDigestSet*)
+  unfold MDCTXInitializedDigestSet, EVP_MD_NNnode; Intros ctxsz.
+  rename H into SZ. rename H0 into SZ1. rename H1 into DSH. forward.
+  forward_if (
+    PROP ( )
+    LOCAL (temp _t'1 (Vint Int.one); temp _ctx ctx)
+    SEP (data_at Tsh (Tstruct _env_md_ctx_st noattr) (d, (nullval, (nullval, nullval))) ctx;
+         data_at dsh (Tstruct _env_md_st noattr) vals d)).
+    { clear H. forward.
+      destruct vals as [tp [mds [flags [ini [upd [fin [blsize ctxsize]]]]]]]; simpl in *; subst.
+      forward. forward. entailer!. simpl; rewrite SZ1; trivial. }
+    { subst; contradiction. }  
+  forward_if (
+    PROP ( )
+    LOCAL (temp _t'2 Vzero; temp _ctx ctx)
+    SEP (data_at Tsh (Tstruct _env_md_ctx_st noattr) (d, (nullval, (nullval, nullval))) ctx;
+         data_at dsh (Tstruct _env_md_st noattr) vals d)). 
+    { clear; forward. forward. entailer!. }
+    { inv H. }
+  forward_if (
+    PROP ( )
+    LOCAL (temp _ctx ctx)
+    SEP (data_at Tsh (Tstruct _env_md_ctx_st noattr) (d, (nullval, (nullval, nullval))) ctx;
+         data_at dsh (Tstruct _env_md_st noattr) vals d)).
+    { elim H; trivial. }
+    { clear H; forward; entailer!. }
+  forward.
+  forward_if (
+    PROP ( )
+    LOCAL (temp _ctx ctx)
+    SEP (data_at Tsh (Tstruct _env_md_ctx_st noattr) (d, (nullval, (nullval, nullval))) ctx;
+         data_at dsh (Tstruct _env_md_st noattr) vals d)).
+    { contradiction. }
+    { clear H; forward; entailer!. }
+  forward_call (ctx). { unfold MDCTXAllocated. cancel. }
+  forward. unfold EVP_MD_NNnode; entailer!.
 + (*ConfiguredOrFinished*)
   Intros nid ctxsz. rename H into SZ. rename H0 into HNID.
   rewrite MDCTXFinished_MDCTXConfigured, orp_dup.
@@ -981,21 +1647,8 @@ Proof.
            (Vint nid, (mds, (flags, (ini, (upd, (fin, (blsize, Vint ctxsz))))))) d));
     [ contradiction | forward; entailer! |].
   forward_call (ctx). { unfold MDCTXAllocated; cancel. }
-  forward. unfold EVP_MD_NNnode; entailer!. 
+  forward. unfold EVP_MD_NNnode; entailer!.
 Time Qed.
-
-Parameter ERR: val -> mpred. 
-Definition OPENSSL_PUT_ERROR_SPEC := DECLARE _ERR_put_error
-  WITH a1:val, a2:val, a3:val, ep:val, a5:val
-  PRE [ 1%positive OF tint, 
-        2%positive OF tint, 3%positive OF tint, 
-        4%positive OF (tptr tschar), 5%positive OF tuint ]
-      PROP() 
-      LOCAL (temp 1%positive a1; temp 2%positive a2; temp 3%positive a3; 
-             temp 4%positive ep; temp 5%positive a5)
-      SEP (ERR ep)
-  POST [ tvoid ]
-    PROP () LOCAL () SEP (ERR ep).
 
 Parameter preInit: Z -> val -> mpred.
 Parameter memblock_preInit: forall i m, memory_block Tsh i m |-- preInit i m.
@@ -1019,11 +1672,10 @@ Definition ini_spec:funspec :=
 
 Inductive EVP_DigestInit_ex_case :=
   Initialized: forall (tsh:share) (vals:reptype (Tstruct _env_md_st noattr)), EVP_DigestInit_ex_case
+(*Adam: InitiatlizedDigestSet case fails!*)
 | HashFinishedEQ: forall (tsh:share) (vals:reptype (Tstruct _env_md_st noattr)), EVP_DigestInit_ex_case
 | HashFinishedNEQ: forall (tsh dsh:share) (vals dvals:reptype (Tstruct _env_md_st noattr)) (d:val), EVP_DigestInit_ex_case.
 
-Definition MDCTXInitialized_MDSET t p : mpred := 
-  data_at Tsh (Tstruct _env_md_ctx_st noattr) (t, (nullval, (nullval, nullval))) p.
 (*
 Axiom Adam1: forall ctx t, 
   field_at Tsh (Tstruct _env_md_ctx_st noattr) [] (t, (nullval, (nullval, nullval))) ctx
@@ -1058,7 +1710,7 @@ end.
 Definition EVP_DigestInit_ex_post (c:EVP_DigestInit_ex_case) (t ctx rv:val): mpred :=
   match c with
     Initialized tsh vals => EVP_MD_NNnode tsh vals t * func_ptr' ini_spec (get_iniptr vals) * 
-          (    (!!(rv=Vzero) && MDCTXInitialized_MDSET t ctx)
+          (    (!!(rv=Vzero) && MDCTXInitializedDigestSet t ctx)
             || (!!(rv=Vone) && EX nid: int, EX ctxsz: int,
                 !!(get_ctxsize vals = Vint ctxsz /\ get_type vals = Vint nid) 
                 && MDCTXConfigured nid ctxsz t ctx) )
@@ -1068,7 +1720,7 @@ Definition EVP_DigestInit_ex_post (c:EVP_DigestInit_ex_case) (t ctx rv:val): mpr
          && MDCTXConfigured nid ctxsz t ctx * EVP_MD_NNnode tsh vals t * func_ptr' ini_spec (get_iniptr vals)
   | HashFinishedNEQ tsh dsh vals dvals d => 
       EVP_MD_NNnode tsh vals t * func_ptr' ini_spec (get_iniptr vals) * EVP_MD_NNnode dsh dvals d *
-        (   (!!(rv=Vzero) && MDCTXInitialized_MDSET t ctx)
+        (   (!!(rv=Vzero) && MDCTXInitializedDigestSet t ctx)
          || (!!(rv=Vone) && EX nid: int, EX ctxsz: int,
              !!(get_ctxsize vals = Vint ctxsz /\ get_type vals = Vint nid) && MDCTXConfigured nid ctxsz t ctx))
 end.
@@ -1150,7 +1802,7 @@ Proof.
         * forward_call (Vint (Int.repr 29), Vint (Int.repr 0), Vint (Int.or (Int.repr 1) (Int.repr 64)),
                  ep, Vint (Int.repr 177)).
           forward. Exists nullval; unfold EVP_MD_NNnode. entailer!.
-          apply orp_right1. unfold MDCTXInitialized_MDSET. cancel.  
+          apply orp_right1. unfold MDCTXInitializedDigestSet. entailer!.
         * intros. unfold POSTCONDITION, abbreviate, overridePost; clear POSTCONDITION.
           old_go_lower. clear H. destruct ek; simpl; normalize. 
       + (*m<>null*)
@@ -1198,7 +1850,7 @@ Proof.
   rename H into TSH. 
   assert (PNt := isptr_is_pointer_or_null _ Pt).
   replace_SEP 3 (MDCTXFinished nid ctxsz t ctx).
-  { entailer!. apply orp_left; [ trivial | Intros data; apply MDCTXHashed_MDCTX_Finished ]. }
+  { entailer!. apply orp_left; [ trivial | Intros data; apply MDCTXHashed_MDCTXFinished ]. }
   rewrite MDCTXFinished_isptr'; Intros.
   unfold MDCTXFinished, EVP_MD_CTX_NNnode; Intros md tp.
   rename H into SZ4. rename H0 into HTP. rename H1 into SZ5.
@@ -1239,7 +1891,7 @@ Proof.
   rename H into TSH. rename H0 into DSH.
   assert (PNt := isptr_is_pointer_or_null _ Pt).
   replace_SEP 4 (MDCTXFinished nid' ctxsz' d ctx).
-  { entailer!. apply orp_left; [ trivial | Intros data; apply MDCTXHashed_MDCTX_Finished ]. }
+  { entailer!. apply orp_left; [ trivial | Intros data; apply MDCTXHashed_MDCTXFinished ]. }
   rewrite MDCTXFinished_isptr'; Intros.
   unfold MDCTXFinished, EVP_MD_CTX_NNnode; Intros md tp.
   rename H into CTXSZ4. rename H0 into HTP. rename H1 into TPSZ.
@@ -1304,7 +1956,7 @@ Proof.
                  ep, Vint (Int.repr 177)).
           forward. Exists nullval; unfold EVP_MD_NNnode; entailer!.
           thaw FR2; cancel. apply orp_right1.
-          unfold MDCTXInitialized_MDSET. cancel.
+          unfold MDCTXInitializedDigestSet. entailer!.
         - inv H. 
         - intros. old_go_lower; clear H. unfold overridePost. if_tac; [ subst; simpl; normalize | trivial ].
       + rewrite memory_block_isptr; Intros. rename H into M.
@@ -1342,9 +1994,52 @@ Proof.
     simpl; forward. Exists (Vint (Int.one)); unfold EVP_MD_NNnode; entailer!.
     thaw Dep. cancel. apply orp_right2. Exists nid ctxsz. entailer!.
     unfold MDCTXConfigured, EVP_MD_CTX_NNnode. Exists m; entailer!.
-    apply Int.eq_false. intros N; subst. 
+    apply Int.eq_false. intros N; subst.
     unfold Int.zero in SZ3; rewrite Int.unsigned_repr in SZ3; omega.
 Time Qed.
+
+(*Here's a failed proof attempt for Init_ex in state MDCTXInitializedDigestSet t, 
+  where t is equal to the type we want to initialize ctx to*)
+Definition EVP_DigestInit_ex_SPEC_MDCTXInitializedDigestSet := DECLARE _EVP_DigestInit_ex
+  WITH ep: val, ctx:val, t:val, e:val, vals:_, nid:int, ctxsz:int, tsh:share
+  PRE [ _ctx OF tptr (Tstruct _env_md_ctx_st noattr), 
+        _type OF tptr (Tstruct _env_md_st noattr),
+        _engine OF tptr (Tstruct _engine_st noattr) ]
+      PROP (get_ctxsize vals = Vint ctxsz; get_type vals = Vint nid;
+            4 <= Int.unsigned ctxsz <= Int.max_unsigned; is_pointer_or_null (get_iniptr vals))
+      LOCAL (gvar ___stringlit_1 ep; temp _type t; temp _ctx ctx; temp _engine e)
+      SEP (ERR ep; EVP_MD_NNnode tsh vals t; func_ptr' ini_spec (get_iniptr vals);
+           MDCTXInitializedDigestSet t ctx)
+  POST [ tint] 
+       PROP () LOCAL ()
+       SEP (). 
+
+Goal semax_body Vprog Gprog_DigestInit_ex f_EVP_DigestInit_ex EVP_DigestInit_ex_SPEC_MDCTXInitializedDigestSet.
+Proof. 
+  start_function. 
+  destruct vals as [tp [mds [flags [ini [upd [fin [blsize ctxsize]]]]]]]; simpl in *. subst.
+  rename H1 into SZ2. rename H2 into Pini.
+  assert (SZ3: Int.unsigned ctxsz > 0) by omega.
+  rewrite EVP_MD_NNnode_isptr'; unfold EVP_MD_NNnode; Intros. rename H into TSH.
+(*  rewrite MDCTXInitializedDigestSet_isptr'; Intros. *)
+  unfold MDCTXInitializedDigestSet; Intros.
+  forward.
+  forward_if (
+    PROP ( )
+    LOCAL (gvar ___stringlit_1 ep; temp _type t; temp _ctx ctx; temp _engine e)
+    SEP (ERR ep; data_at tsh (Tstruct _env_md_st noattr)
+                  (Vint nid, (mds, (flags, (ini, (upd, (fin, (blsize, Vint ctxsz))))))) t;
+         func_ptr' ini_spec ini;
+         data_at Tsh (Tstruct _env_md_ctx_st noattr) (t, (nullval, (nullval, nullval))) ctx)).
+  { apply ptr_comp_Cne_t in H; try congruence; destruct t; try contradiction; trivial. }
+  { clear H. forward; entailer!. } 
+  forward. forward.
+(*    replace_SEP 4 (preInit (Int.unsigned ctxsz) m). { entailer!. apply memblock_preInit. } *)
+  forward_call (ctx, Tsh, (t, (nullval, (nullval, nullval))), tsh, 
+                   (Vint nid, (mds, (flags, (ini, (upd, (fin, (blsize, Vint ctxsz))))))), 
+                   ctxsz, nid).
+      { simpl. admit. }
+Admitted.
 
 Definition EVP_DigestInit_SPEC := DECLARE _EVP_DigestInit
   WITH ep: val, ctx:val, t:val, tsh:share, 
@@ -1361,7 +2056,7 @@ Definition EVP_DigestInit_SPEC := DECLARE _EVP_DigestInit
   POST [ tint] EX rv:_,
        PROP ()
        LOCAL (temp ret_temp rv)
-       SEP ((!!(rv=Vzero) && MDCTXInitialized_MDSET t ctx)
+       SEP ((!!(rv=Vzero) && MDCTXInitializedDigestSet t ctx)
             || (!!(rv=Vone) && MDCTXConfigured nid ctxsz t ctx);
             ERR ep; EVP_MD_NNnode tsh vals t; func_ptr' ini_spec (get_iniptr vals)).
 
@@ -1553,7 +2248,7 @@ Proof.
   forward. cancel.
 Qed.
 
-(*Adam2: State MDCTXAlocated must be ruled out, ie if ictx is nonnull, 
+(*Adam2: State MDCTXAllocated ictx must be ruled out, ie if ictx is nonnull, 
   it must also be initialized already. Otherwise the access to 
   in -> digest in the first conditional will access a Vundef.
   (Alternative: we change the def of Allocated...)
@@ -1563,7 +2258,7 @@ Definition EVP_MD_CTX_copy_ex_SPEC_Allocated := DECLARE _EVP_MD_CTX_copy_ex
         _in OF (tptr (Tstruct _env_md_ctx_st noattr)) ]
       PROP ()
       LOCAL (gvar ___stringlit_1 ep; temp _out octx; temp _in ictx)
-      SEP (ERR ep;(* copyExPre case ictx octx*)MDCTXAllocated ictx)
+      SEP (ERR ep;MDCTXAllocated ictx)
   POST [ tint] EX rv:_,
        PROP ()
        LOCAL (temp ret_temp rv)
@@ -1592,13 +2287,1096 @@ Proof.
 Definition Gprog_copy_ex : funspecs :=
   (*FAILS TO TERMINATE: ltac:(with_library prog [EVP_MD_type_SPEC]). *)
   [EVP_MD_CTX_cleanup_SPEC; OPENSSL_PUT_ERROR_SPEC; OPENSSL_malloc_SPEC; OPENSSL_memcpy_STRONGSPEC ].
-(*note use of strongspec here! Without it, we'd have to prove a leema like the following (and maybe its inverse)
+(*note use of strongspec here! Without it, we'd have to prove a lemma like the following (and maybe its inverse)
   (Of course, such a lemma may be needed to justify memcpy strongspec...
 Lemma DigestRep_changeREP tp v data md
   (D: DigestRep tp v (map Int.unsigned data)):
   data_at Tsh tp v md = data_at Tsh (tarray tuchar (sizeof tp)) (map Vint data) md.
 Admitted.*)
 
+Inductive EVP_MD_CTX_copy_case :=
+  CopyInitialized: EVP_MD_CTX_copy_case
+| CopyHashedFinished: forall (dsh:share) (vals:reptype (Tstruct _env_md_st noattr))
+                             (data: option (list int)) (d:val), EVP_MD_CTX_copy_case.
+
+Definition EVP_MD_CTX_copy_pre (c:EVP_MD_CTX_copy_case) (octx ictx:val) : mpred :=
+  match c with
+   CopyInitialized => MDCTXInitialized ictx
+ | CopyHashedFinished dsh vals data d => 
+     EX nid:int, EX ctxsz:int, 
+     !!(get_ctxsize vals = Vint ctxsz /\ 4 <= Int.unsigned ctxsz <= Int.max_unsigned)
+     && match data with None => MDCTXFinished nid ctxsz d ictx
+                     | Some v => MDCTXHashed nid ctxsz (map Int.unsigned v) d ictx
+        end * 
+        EVP_MD_NNnode dsh vals d * MDCTXInitialized octx
+ end.
+
+Definition EVP_MD_CTX_copy_post (c:EVP_MD_CTX_copy_case) (octx ictx rv:val) : mpred :=
+  match c with
+   CopyInitialized => !!(rv=nullval)&& MDCTXInitialized ictx
+ | CopyHashedFinished dsh vals data d => 
+     EX nid:int, EX ctxsz:int, 
+     !!(get_ctxsize vals = Vint ctxsz /\ 4 <= Int.unsigned ctxsz <= Int.max_unsigned)
+     && match data with None => MDCTXFinished nid ctxsz d ictx
+                     | Some v => MDCTXHashed nid ctxsz (map Int.unsigned v) d ictx
+        end * EVP_MD_NNnode dsh vals d *
+        ( (!!(rv=nullval) && MDCTXInitializedDigestSet d octx)
+          || (!!(rv=Vone) && match data with None => MDCTXFinished nid ctxsz d octx
+                                           | Some v => MDCTXHashed nid ctxsz (map Int.unsigned v) d octx
+                             end ))
+ end.
+
+Definition EVP_MD_CTX_copy_ex_SPEC := DECLARE _EVP_MD_CTX_copy_ex
+  WITH ep: val, octx:val, ictx:val, c: EVP_MD_CTX_copy_case
+  PRE [ _out OF (tptr (Tstruct _env_md_ctx_st noattr)),
+        _in OF (tptr (Tstruct _env_md_ctx_st noattr)) ]
+      PROP ()
+      LOCAL (gvar ___stringlit_1 ep; temp _out octx; temp _in ictx)
+      SEP (ERR ep; EVP_MD_CTX_copy_pre c octx ictx)
+  POST [ tint] EX rv:val,
+       PROP ()
+       LOCAL (temp ret_temp rv)
+       SEP (ERR ep; EVP_MD_CTX_copy_post c octx ictx rv).
+
+Lemma body_EVP_MD_CTX_copy_ex: semax_body Vprog Gprog_copy_ex f_EVP_MD_CTX_copy_ex EVP_MD_CTX_copy_ex_SPEC.
+Proof. 
+  start_function. forward. destruct c; simpl.
++ (*Initialized*)
+  rewrite MDCTXInitialized_isptr' with (p:=ictx); Intros.
+  (*  rewrite MDCTXInitialized_isptr' with (p:=octx); Intros.*)
+  forward_if (
+    PROP ( )
+     LOCAL (temp _t'1 Vone; temp _tmp_buf (Vint (Int.repr 0));
+            gvar ___stringlit_1 ep; temp _out octx; temp _in ictx)
+     SEP (ERR ep; (*MDCTXInitialized octx;*) MDCTXInitialized ictx)).
+  { clear H; 
+    apply denote_tc_test_eq_split; try apply valid_pointer_null.
+    apply sepcon_valid_pointer2. apply MDCTXInitialized_valid_ptr. }
+  { subst; contradiction. } 
+  { unfold MDCTXInitialized. forward. forward. entailer!. }
+  forward_if (PROP (False) LOCAL () SEP ()).
+  { forward_call (Vint (Int.repr 29), Vint (Int.repr 0), Vint (Int.repr 100),
+                 ep, Vint (Int.repr 121)).
+    forward. Exists nullval; entailer!. }
+  { inv H. }
+  normalize.
++ (*HashedFinished*)
+  Intros nid ctxsz. rename H into SZ. rename H0 into SZ1.
+  rewrite MDCTXInitialized_isptr'; Intros.
+  assert_PROP (isptr ictx) as Pictx by
+    ( destruct data; [ rewrite MDCTXHashed_isptr'; entailer! | rewrite MDCTXFinished_isptr'; entailer! ] ).
+  rewrite EVP_MD_NNnode_isptr'; Intros.
+  forward_if (
+    PROP ( )
+     LOCAL (temp _t'1 Vzero; temp _tmp_buf (Vint (Int.repr 0));
+            gvar ___stringlit_1 ep; temp _out octx; temp _in ictx)
+     SEP (ERR ep; MDCTXInitialized octx; 
+          match data with
+   | Some v => MDCTXHashed nid ctxsz (map Int.unsigned v) d ictx
+   | None => MDCTXFinished nid ctxsz d ictx
+   end (*MDCTXHashed nid ctxsz (map Int.unsigned data) d ictx*); EVP_MD_NNnode dsh vals d)).
+  { clear H; 
+    apply denote_tc_test_eq_split; try apply valid_pointer_null.
+    apply sepcon_valid_pointer1. apply sepcon_valid_pointer1. 
+    apply sepcon_valid_pointer2.
+    destruct data; [ apply MDCTXHashed_valid_ptr | apply MDCTXFinished_valid_ptr ]. }
+  { subst; contradiction. } 
+  { clear H. unfold EVP_MD_NNnode; Intros. rename H into DSH. 
+    destruct data. 
+    + unfold MDCTXHashed, EVP_MD_CTX_NNnode. Intros md tp v.
+      forward. forward. entailer!.
+      - simpl. destruct d; try contradiction; simpl; trivial.
+      - unfold MDCTXHashed, EVP_MD_NNnode, EVP_MD_CTX_NNnode. Exists md tp v; entailer!.
+    + unfold MDCTXFinished, EVP_MD_CTX_NNnode. Intros md tp.
+      forward. forward. entailer!.
+      - simpl. destruct d; try contradiction; simpl; trivial.
+      - unfold MDCTXFinished, EVP_MD_NNnode, EVP_MD_CTX_NNnode. Exists md tp; entailer!.
+  }
+  forward_if (
+    PROP ( )
+    LOCAL (temp _tmp_buf (Vint (Int.repr 0));
+           gvar ___stringlit_1 ep; temp _out octx; temp _in ictx)
+    SEP (ERR ep; MDCTXInitialized octx; 
+         match data with
+         | Some v => MDCTXHashed nid ctxsz (map Int.unsigned v) d ictx
+         | None => MDCTXFinished nid ctxsz d ictx
+         end;
+         EVP_MD_NNnode dsh vals d)).
+  { elim H; trivial. }
+  { clear H; forward; entailer!. }
+  unfold MDCTXInitialized. forward.
+  destruct data.
+  - (*Hashed*)
+    unfold MDCTXHashed; unfold EVP_MD_CTX_NNnode. Intros md tp v.
+    rename H into SZ2. rename H0 into HTP. rename H1 into SZ3. rename H2 into V.
+  rewrite data_at_isptr with (p:=md); Intros.
+  forward.
+  forward_if (
+    PROP ( )
+    LOCAL (temp _tmp_buf (Vint (Int.repr 0)); gvar ___stringlit_1 ep;
+           temp _out octx; temp _in ictx)
+    SEP (ERR ep; EVP_MD_NNnode dsh vals d;
+         data_at Tsh (Tstruct _env_md_ctx_st noattr) (nullval, (nullval, (nullval, nullval))) octx;
+         data_at Tsh (Tstruct _env_md_ctx_st noattr) (d, (md, (nullval, nullval))) ictx;
+         data_at Tsh tp v md)).
+  { clear H.
+    apply denote_tc_test_eq_split; try apply valid_pointer_null.
+    apply sepcon_valid_pointer2. apply EVP_MD_NNnode_validptr. }
+  { apply ptr_comp_Ceq_t in H; simpl; trivial; subst; contradiction. }
+  { clear H. forward; entailer!. }
+  forward_call (octx, ClInitialized).
+  { simpl; unfold MDCTXInitialized; entailer!. }
+  forward. simpl; unfold MDCTXInitialized. forward.
+  simpl. rewrite sem_cast_neutral_ptr; simpl; trivial.
+  forward.
+  forward_if (
+    PROP ( )
+    LOCAL (temp _t'3 Vone; temp _tmp_buf (Vint (Int.repr 0));
+           gvar ___stringlit_1 ep; temp _out octx; temp _in ictx)
+    SEP (data_at Tsh (Tstruct _env_md_ctx_st noattr) (d, (nullval, (nullval, nullval))) octx; 
+         ERR ep; data_at Tsh tp v md; EVP_MD_NNnode dsh vals d;
+         data_at Tsh (Tstruct _env_md_ctx_st noattr) (d, (md, (nullval, nullval))) ictx)).
+  { clear H. 
+    apply denote_tc_test_eq_split; try apply valid_pointer_null.
+    apply sepcon_valid_pointer2. apply data_at_valid_ptr; [intuition | omega ]. }
+  { clear H. forward. 
+    unfold EVP_MD_NNnode; Intros. rename H into TSH.
+    destruct vals as [tpp [mds [flags [ini [upd [fin [blsize ctxsize]]]]]]]; simpl in *; subst.
+    forward. forward. entailer!. simpl. rewrite SZ2; trivial. 
+    unfold EVP_MD_NNnode; entailer!. }
+  { subst md; contradiction. }
+  forward_if (
+    PROP ( )
+    LOCAL (gvar ___stringlit_1 ep; temp _out octx; temp _in ictx)
+    SEP (ERR ep; data_at Tsh tp v md; EVP_MD_NNnode dsh vals d;
+         EX m :_, (!!(malloc_compatible (Int.unsigned ctxsz) m) 
+             && data_at Tsh (Tstruct _env_md_ctx_st noattr) (d, (m, (nullval, nullval))) octx * 
+                data_at Tsh tp v m);
+         data_at Tsh (Tstruct _env_md_ctx_st noattr)
+            (d, (md, (nullval, nullval))) ictx));
+  [ clear H | inv H | ].
+  { forward_if (
+    PROP ( )
+    LOCAL (gvar ___stringlit_1 ep; temp _out octx; temp _in ictx)
+    SEP (ERR ep; data_at Tsh tp v md; EVP_MD_NNnode dsh vals d;
+         EX m :_, (!!(malloc_compatible (Int.unsigned ctxsz) m) 
+             && data_at Tsh (Tstruct _env_md_ctx_st noattr) (d, (m, (nullval, nullval))) octx * 
+                memory_block Tsh (Int.unsigned ctxsz) m);
+         data_at Tsh (Tstruct _env_md_ctx_st noattr)
+            (d, (md, (nullval, nullval))) ictx));
+    [ contradiction | clear H |].
+    { forward. unfold EVP_MD_NNnode; Intros. rename H into TSH.
+      destruct vals as [tpp [mds [flags [ini [upd [fin [blsize ctxsize]]]]]]]; simpl in *; subst.
+      forward.
+      forward_call (Int.unsigned ctxsz). simpl; rewrite Int.repr_unsigned; apply prop_right; trivial.
+      Intros m. forward. forward.
+      apply semax_orp_SEPx; Intros.
+      + (*m=Null*)
+        subst; simpl.
+        forward_if ( PROP (False) LOCAL () SEP ()).
+        - clear H.
+          forward_call (Vint (Int.repr 29), Vint (Int.repr 0), Vint (Int.or (Int.repr 1) (Int.repr 64)),
+                 ep, Vint (Int.repr 142)).
+          forward. Exists nullval. entailer!. unfold MDCTXHashed, EVP_MD_NNnode.
+          Exists nid ctxsz md tp v; unfold EVP_MD_CTX_NNnode; entailer!.
+          apply orp_right1. unfold MDCTXInitializedDigestSet. entailer!.
+        - inv H.
+        - intros. unfold POSTCONDITION, abbreviate, overridePost; clear POSTCONDITION.
+          old_go_lower. clear H. destruct ek; simpl; normalize. 
+      + (*m<>null*)
+        rename H into M. 
+        rewrite memory_block_isptr; Intros.
+        rewrite eval_cast_neutral_isptr; simpl; trivial.
+        forward_if (
+          PROP ( )
+          LOCAL (gvar ___stringlit_1 ep; temp _out octx; temp _in ictx)
+          SEP (memory_block Tsh (Int.unsigned ctxsz) m;
+               data_at Tsh (Tstruct _env_md_ctx_st noattr) (d, (m, (nullval, nullval))) octx; 
+               ERR ep; data_at Tsh tp v md;
+               data_at dsh (Tstruct _env_md_st noattr) (tpp, (mds, (flags, (ini, (upd, (fin, (blsize, Vint ctxsz))))))) d;
+               data_at Tsh (Tstruct _env_md_ctx_st noattr) (d, (md, (nullval, nullval))) ictx)).
+        - clear H.
+          apply denote_tc_test_eq_split; [ apply sepcon_valid_pointer1 | apply valid_pointer_null].
+          apply sepcon_valid_pointer1. apply sepcon_valid_pointer1. apply sepcon_valid_pointer1.
+          apply sepcon_valid_pointer1. apply memory_block_valid_ptr. intuition. omega.
+        - destruct m; try contradiction. simpl in H. inv H.
+        - clear H. forward. entailer!.
+        - intros. unfold POSTCONDITION, abbreviate, overridePost; clear POSTCONDITION.
+          old_go_lower. clear H. destruct ek; simpl; normalize. entailer!. 
+          Exists m; unfold EVP_MD_NNnode; entailer!. }
+    Intros m. rename H into M. forward. forward. forward.
+    unfold EVP_MD_NNnode; Intros. rename H into TSH. 
+    destruct vals as [tpp [mds [flags [ini [upd [fin [blsize ctxsize]]]]]]]; simpl in *; subst.
+    forward. (*
+    rewrite (DigestRep_changeREP tp v data); trivial.
+    replace_SEP  1 (data_at Tsh (tarray tuchar (Int.unsigned ctxsz)) (map Vint data) md).
+    { entailer!. rewrite <- SZ3; trivial. } 
+    forward_call ((Tsh,Tsh),m, md,Int.unsigned ctxsz, data).
+         { rewrite Int.repr_unsigned; entailer!. }
+         { simpl. cancel. }
+         { simpl; split; trivial. intuition. split; trivial. apply Int.unsigned_range_2. }
+    entailer!. Exists m; unfold EVP_MD_NNnode.
+    rewrite ! (DigestRep_changeREP tp v data); trivial.
+    entailer!. rewrite <- ! SZ3. cancel. }*)
+
+    forward_call ((Tsh,Tsh),m, md,Int.unsigned ctxsz, Build_REPTYPE tp v). 
+         { rewrite Int.repr_unsigned; entailer!. }
+         { simpl. cancel. }
+         { simpl; split; trivial. intuition. split; trivial. 
+           split. apply Int.unsigned_range_2. rewrite SZ3; trivial. }
+    entailer!. Exists m; unfold EVP_MD_NNnode; entailer!. }
+
+  Intros m. rename H into M. forward. forward. forward. 
+  forward_if (
+    PROP ( )
+    LOCAL (temp _t'5 (Vint (Int.repr 0)); gvar ___stringlit_1 ep; temp _out octx; temp _in ictx)
+    SEP (ERR ep; data_at Tsh tp v md; EVP_MD_NNnode dsh vals d;
+         data_at Tsh (Tstruct _env_md_ctx_st noattr) (d, (m, (nullval, Vint Int.zero))) octx;
+         data_at Tsh tp v m;
+         data_at Tsh (Tstruct _env_md_ctx_st noattr) (d, (md, (nullval, nullval))) ictx)).
+  { contradiction. }
+  { clear H. forward. entailer!. }
+  forward_if (
+    PROP ( )
+    LOCAL (gvar ___stringlit_1 ep; temp _out octx; temp _in ictx)
+    SEP (ERR ep; data_at Tsh tp v md; EVP_MD_NNnode dsh vals d;
+         data_at Tsh (Tstruct _env_md_ctx_st noattr) (d, (m, (nullval, Vint Int.zero))) octx;
+         data_at Tsh tp v m;
+         data_at Tsh (Tstruct _env_md_ctx_st noattr) (d, (md, (nullval, nullval))) ictx)).
+  { contradiction. }
+  { clear H. forward. entailer!. }
+  forward. Exists Vone; unfold MDCTXHashed; entailer!.
+  Exists nid ctxsz md tp v. unfold EVP_MD_CTX_NNnode; entailer!.
+  apply orp_right2. Exists m tp v; entailer!.
+
+  - (*Finished*)
+  unfold MDCTXFinished, EVP_MD_CTX_NNnode; Intros md tp.
+  rename H into SZ2. rename H0 into HTP. rename H1 into SZ3.
+  rewrite data_at__isptr with (p:=md); Intros.
+  forward.
+  forward_if (
+    PROP ( )
+    LOCAL (temp _tmp_buf (Vint (Int.repr 0)); gvar ___stringlit_1 ep;
+           temp _out octx; temp _in ictx)
+    SEP (ERR ep; EVP_MD_NNnode dsh vals d;
+         data_at Tsh (Tstruct _env_md_ctx_st noattr) (nullval, (nullval, (nullval, nullval))) octx;
+         data_at Tsh (Tstruct _env_md_ctx_st noattr) (d, (md, (nullval, nullval))) ictx;
+         data_at_ Tsh tp md)).
+  { clear H.
+    apply denote_tc_test_eq_split; try apply valid_pointer_null.
+    apply sepcon_valid_pointer2. apply EVP_MD_NNnode_validptr. }
+  { apply ptr_comp_Ceq_t in H; simpl; trivial; subst; contradiction. }
+  { clear H. forward; entailer!. }
+  forward_call (octx, ClInitialized).
+  { simpl; unfold MDCTXInitialized; entailer!. }
+  forward. simpl; unfold MDCTXInitialized. forward.
+  simpl. rewrite sem_cast_neutral_ptr; simpl; trivial.
+  forward.
+  forward_if (
+    PROP ( )
+    LOCAL (temp _t'3 Vone; temp _tmp_buf (Vint (Int.repr 0));
+           gvar ___stringlit_1 ep; temp _out octx; temp _in ictx)
+    SEP (data_at Tsh (Tstruct _env_md_ctx_st noattr) (d, (nullval, (nullval, nullval))) octx; 
+         ERR ep; data_at_ Tsh tp md; EVP_MD_NNnode dsh vals d;
+         data_at Tsh (Tstruct _env_md_ctx_st noattr) (d, (md, (nullval, nullval))) ictx)).
+  { clear H. 
+    apply denote_tc_test_eq_split; try apply valid_pointer_null.
+    apply sepcon_valid_pointer2. apply data_at_valid_ptr; [intuition | omega ]. }
+  { clear H. forward. 
+    unfold EVP_MD_NNnode; Intros. rename H into TSH.
+    destruct vals as [tpp [mds [flags [ini [upd [fin [blsize ctxsize]]]]]]]; simpl in *; subst.
+    forward. forward. entailer!. simpl. rewrite SZ2; trivial. 
+    unfold EVP_MD_NNnode; entailer!. }
+  { subst md; contradiction. }
+  forward_if (
+    PROP ( )
+    LOCAL (gvar ___stringlit_1 ep; temp _out octx; temp _in ictx)
+    SEP (ERR ep; data_at_ Tsh tp md; EVP_MD_NNnode dsh vals d;
+         EX m :_, (!!(malloc_compatible (Int.unsigned ctxsz) m) 
+             && data_at Tsh (Tstruct _env_md_ctx_st noattr) (d, (m, (nullval, nullval))) octx * 
+                data_at_ Tsh tp m);
+         data_at Tsh (Tstruct _env_md_ctx_st noattr) (d, (md, (nullval, nullval))) ictx));
+  [ clear H | inv H | ].
+  { forward_if (
+    PROP ( )
+    LOCAL (gvar ___stringlit_1 ep; temp _out octx; temp _in ictx)
+    SEP (ERR ep; data_at_ Tsh tp md; EVP_MD_NNnode dsh vals d;
+         EX m :_, (!!(malloc_compatible (Int.unsigned ctxsz) m) 
+             && data_at Tsh (Tstruct _env_md_ctx_st noattr) (d, (m, (nullval, nullval))) octx * 
+                memory_block Tsh (Int.unsigned ctxsz) m);
+         data_at Tsh (Tstruct _env_md_ctx_st noattr) (d, (md, (nullval, nullval))) ictx));
+    [ contradiction | clear H |].
+    { forward. unfold EVP_MD_NNnode; Intros. rename H into TSH.
+      destruct vals as [tpp [mds [flags [ini [upd [fin [blsize ctxsize]]]]]]]; simpl in *; subst.
+      forward.
+      forward_call (Int.unsigned ctxsz). simpl; rewrite Int.repr_unsigned; apply prop_right; trivial.
+      Intros m. forward. forward.
+      apply semax_orp_SEPx; Intros.
+      + (*m=Null*)
+        subst; simpl.
+        forward_if ( PROP (False) LOCAL () SEP ()).
+        - clear H.
+          forward_call (Vint (Int.repr 29), Vint (Int.repr 0), Vint (Int.or (Int.repr 1) (Int.repr 64)),
+                 ep, Vint (Int.repr 142)).
+          forward. Exists nullval. entailer!. unfold MDCTXFinished, EVP_MD_NNnode.
+          Exists nid ctxsz md tp; unfold EVP_MD_CTX_NNnode; entailer!.
+          apply orp_right1. unfold MDCTXInitializedDigestSet. entailer!.
+        - inv H.
+        - intros. unfold POSTCONDITION, abbreviate, overridePost; clear POSTCONDITION.
+          old_go_lower. clear H. destruct ek; simpl; normalize. 
+      + (*m<>null*)
+        rename H into M. 
+        rewrite memory_block_isptr; Intros.
+        rewrite eval_cast_neutral_isptr; simpl; trivial.
+        forward_if (
+          PROP ( )
+          LOCAL (gvar ___stringlit_1 ep; temp _out octx; temp _in ictx)
+          SEP (memory_block Tsh (Int.unsigned ctxsz) m;
+               data_at Tsh (Tstruct _env_md_ctx_st noattr) (d, (m, (nullval, nullval))) octx; 
+               ERR ep; data_at_ Tsh tp md;
+               data_at dsh (Tstruct _env_md_st noattr) (tpp, (mds, (flags, (ini, (upd, (fin, (blsize, Vint ctxsz))))))) d;
+               data_at Tsh (Tstruct _env_md_ctx_st noattr) (d, (md, (nullval, nullval))) ictx)).
+        - clear H.
+          apply denote_tc_test_eq_split; [ apply sepcon_valid_pointer1 | apply valid_pointer_null].
+          apply sepcon_valid_pointer1. apply sepcon_valid_pointer1. apply sepcon_valid_pointer1.
+          apply sepcon_valid_pointer1. apply memory_block_valid_ptr. intuition. omega.
+        - destruct m; try contradiction. simpl in H. inv H.
+        - clear H. forward. entailer!.
+        - intros. unfold POSTCONDITION, abbreviate, overridePost; clear POSTCONDITION.
+          old_go_lower. clear H. destruct ek; simpl; normalize. entailer!. 
+          Exists m; unfold EVP_MD_NNnode; entailer!. }
+    Intros m. rename H into M. forward. forward. forward.
+    unfold EVP_MD_NNnode; Intros. rename H into TSH. 
+    destruct vals as [tpp [mds [flags [ini [upd [fin [blsize ctxsize]]]]]]]; simpl in *; subst.
+    forward. 
+    replace_SEP 1 (data_at Tsh tp (default_val tp) md) by entailer!.
+    forward_call ((Tsh,Tsh),m, md, Int.unsigned ctxsz, Build_REPTYPE tp (default_val tp)).
+         { rewrite Int.repr_unsigned; entailer!. }
+         { simpl. cancel. }
+         { simpl; split; trivial. intuition. split; trivial.
+           split. apply Int.unsigned_range_2. rewrite SZ3; trivial. }
+    entailer!. Exists m; unfold EVP_MD_NNnode; entailer!. }
+  Intros m. rename H into M. forward. forward. forward. 
+  forward_if (
+    PROP ( )
+    LOCAL (temp _t'5 (Vint (Int.repr 0)); gvar ___stringlit_1 ep; temp _out octx; temp _in ictx)
+    SEP (ERR ep; data_at_ Tsh tp md; EVP_MD_NNnode dsh vals d;
+         data_at Tsh (Tstruct _env_md_ctx_st noattr) (d, (m, (nullval, Vint Int.zero))) octx;
+         data_at_ Tsh tp m;
+         data_at Tsh (Tstruct _env_md_ctx_st noattr) (d, (md, (nullval, nullval))) ictx)).
+  { contradiction. }
+  { clear H. forward. entailer!. }
+  forward_if (
+    PROP ( )
+    LOCAL (gvar ___stringlit_1 ep; temp _out octx; temp _in ictx)
+    SEP (ERR ep; data_at_ Tsh tp md; EVP_MD_NNnode dsh vals d;
+         data_at Tsh (Tstruct _env_md_ctx_st noattr) (d, (m, (nullval, Vint Int.zero))) octx;
+         data_at_ Tsh tp m;
+         data_at Tsh (Tstruct _env_md_ctx_st noattr) (d, (md, (nullval, nullval))) ictx)).
+  { contradiction. }
+  { clear H. forward. entailer!. }
+  forward. Exists Vone; unfold MDCTXFinished; entailer!.
+  Exists nid ctxsz md tp. unfold EVP_MD_CTX_NNnode; entailer!.
+  apply orp_right2. Exists m tp; entailer!.
+Time Qed.
+
+(*Also supports Hashed octx, since Hashed octx |-- Finished octx. (BUT THAT'S NOT EXPOSED!
+  Allocation is performed, and result may be Vone or Vnull*)
+Definition EVP_MD_CTX_copy_ex_SPEC_Finished_NEQ := DECLARE _EVP_MD_CTX_copy_ex
+  WITH ep: val, octx:val, ictx:val,
+       nid:int, ctxsz:int, sh:share * share, vals:_, t:val,
+       nid':int, ctxsz':int, d:val
+  PRE [ _out OF (tptr (Tstruct _env_md_ctx_st noattr)),
+        _in OF (tptr (Tstruct _env_md_ctx_st noattr)) ]
+      PROP (get_ctxsize (snd vals) = Vint ctxsz' /\ get_type (snd vals) = Vint nid';
+            get_ctxsize (fst vals) = Vint ctxsz; 4 <= Int.unsigned ctxsz <= Int.max_unsigned; d<>t)
+      LOCAL (gvar ___stringlit_1 ep; temp _out octx; temp _in ictx)
+      SEP (ERR ep; MDCTXFinished nid' ctxsz' d octx; 
+           MDCTXFinished nid ctxsz t ictx;
+           EVP_MD_NNnode (fst sh) (fst vals) t; EVP_MD_NNnode (snd sh) (snd vals) d)
+  POST [ tint] EX rv:_,
+       PROP ()
+       LOCAL (temp ret_temp rv)
+       SEP (ERR ep; MDCTXFinished nid ctxsz t ictx; 
+            EVP_MD_NNnode (fst sh) (fst vals) t; EVP_MD_NNnode (snd sh) (snd vals) d;
+            (!!(rv=nullval) && MDCTXInitializedDigestSet t octx) 
+            || (!!(rv=Vone) && MDCTXFinished nid ctxsz t octx)).
+
+(*Also supports Hashed octx, since Hashed octx |-- Finished octx.
+  No allocation is performed, and result value is always Vone*)
+Definition EVP_MD_CTX_copy_ex_SPEC_Finished_EQ := DECLARE _EVP_MD_CTX_copy_ex
+  WITH ep: val, octx:val, ictx:val,
+       nid:int, ctxsz:int, tsh:share, vals:_, t:val
+  PRE [ _out OF (tptr (Tstruct _env_md_ctx_st noattr)),
+        _in OF (tptr (Tstruct _env_md_ctx_st noattr)) ]
+      PROP (get_ctxsize vals = Vint ctxsz; 4 <= Int.unsigned ctxsz <= Int.max_unsigned)
+      LOCAL (gvar ___stringlit_1 ep; temp _out octx; temp _in ictx)
+      SEP (ERR ep; MDCTXFinished nid ctxsz t octx; 
+           MDCTXFinished nid ctxsz t ictx;
+           EVP_MD_NNnode tsh vals t)
+  POST [ tint] 
+       PROP ()
+       LOCAL (temp ret_temp Vone)
+       SEP (ERR ep; MDCTXFinished nid ctxsz t ictx; EVP_MD_NNnode tsh vals t;
+            MDCTXFinished nid ctxsz t octx).
+
+Lemma body_EVP_MD_CTX_copy_ex_Finished_NEQ: semax_body Vprog Gprog_copy_ex f_EVP_MD_CTX_copy_ex EVP_MD_CTX_copy_ex_SPEC_Finished_NEQ.
+Proof. 
+  start_function. destruct H as [SZ' NID'].
+  rename H0 into SZ. rename H1 into SZ1. rename H2 into DT. forward.
+  rewrite MDCTXFinished_isptr' with (p:=ictx); Intros.
+  rewrite MDCTXFinished_isptr' with (p:=octx); Intros.
+  rewrite EVP_MD_NNnode_isptr' with (p:= t); Intros.
+  rewrite EVP_MD_NNnode_isptr' with (p:= d); Intros.
+  destruct sh as [tsh dsh]. destruct vals as [tvals dvals]; simpl in *.
+  destruct tvals as [tpp [mds [flags [ini [upd [fin [blsize ctxsize]]]]]]]; simpl in *; subst.
+  freeze [0;1;4] FR1.
+  forward_if (
+    PROP ( )
+     LOCAL (temp _t'1 Vzero; temp _tmp_buf (Vint (Int.repr 0));
+            gvar ___stringlit_1 ep; temp _out octx; temp _in ictx)
+     SEP (FRZL FR1; MDCTXFinished nid ctxsz t ictx;
+          EVP_MD_NNnode tsh (*tvals*)(tpp, (mds, (flags, (ini, (upd, (fin, (blsize, Vint ctxsz))))))) t)).
+  { clear H; 
+    apply denote_tc_test_eq_split; try apply valid_pointer_null.
+    apply sepcon_valid_pointer1. 
+    apply sepcon_valid_pointer2. apply MDCTXFinished_valid_ptr. }
+  { subst; contradiction. } 
+  { clear H. unfold MDCTXFinished. unfold EVP_MD_CTX_NNnode. Intros md tp.
+    unfold EVP_MD_NNnode; Intros.
+    forward. forward. entailer!.
+    + destruct t; try contradiction; simpl; trivial.
+    + unfold MDCTXFinished, EVP_MD_NNnode, EVP_MD_CTX_NNnode. Exists md tp; entailer!. }
+  forward_if (
+    PROP ( )
+    LOCAL (temp _tmp_buf (Vint (Int.repr 0));
+           gvar ___stringlit_1 ep; temp _out octx; temp _in ictx)
+    SEP (FRZL FR1; MDCTXFinished nid ctxsz t ictx;
+         EVP_MD_NNnode tsh (*tvals*)(tpp, (mds, (flags, (ini, (upd, (fin, (blsize, Vint ctxsz))))))) t)).
+  { elim H; trivial. }
+  { clear H; forward; entailer!. }
+  thaw FR1.
+      unfold MDCTXFinished,EVP_MD_CTX_NNnode. Intros md' tp' md tp.
+      rename H into SZ2'. rename H0 into TP'. rename H1 into SZ3'. (* rename H2 into V'.*)
+      rename H2 into SZ2. rename H3 into TP. rename H4 into SZ3.
+      rewrite data_at__isptr with (p:=md); Intros.
+      rewrite data_at__isptr with (p:=md'); Intros.
+      forward. forward.
+      forward_if (
+        PROP ( )
+        LOCAL (temp _tmp_buf (Vint (Int.repr 0)); gvar ___stringlit_1 ep;
+               temp _out octx; temp _in ictx)
+        SEP (ERR ep;
+             data_at Tsh (Tstruct _env_md_ctx_st noattr) (d, (md', (nullval, nullval))) octx;
+             data_at_ Tsh tp' md'; EVP_MD_NNnode dsh dvals d;
+             data_at Tsh (Tstruct _env_md_ctx_st noattr) (t, (md, (nullval, nullval))) ictx;
+             data_at_ Tsh tp md; EVP_MD_NNnode tsh (*tvals*)(tpp, (mds, (flags, (ini, (upd, (fin, (blsize, Vint ctxsz))))))) t)).
+      { clear H.
+        apply denote_tc_test_eq_split; 
+        [ apply sepcon_valid_pointer1 | apply sepcon_valid_pointer2; apply EVP_MD_NNnode_validptr ].
+        apply sepcon_valid_pointer1; apply sepcon_valid_pointer1. apply sepcon_valid_pointer2; apply EVP_MD_NNnode_validptr. }
+      { apply ptr_comp_Ceq_t in H; trivial; simpl in H. congruence. }
+      { forward; entailer!. }
+  gather_SEP 1 2.
+  replace_SEP 0 (MDCTXConfigured nid' ctxsz' d octx || MDCTXFinished nid' ctxsz' d octx).
+  { unfold MDCTXFinished; entailer!. apply orp_right2. Exists md' tp'; entailer!. }
+  forward_call (octx, ClConfiguredOrFinished dsh dvals d).
+  { simpl. Exists nid' ctxsz'; entailer!. }
+  simpl. normalize.
+  rewrite data_at__isptr with (p:=md); Intros.
+  forward. simpl; unfold MDCTXInitialized; Intros. forward.
+  simpl. rewrite sem_cast_neutral_ptr; simpl; trivial.
+  forward. freeze [0;1;2] FR1.
+  forward_if (
+    PROP ( )
+    LOCAL (temp _t'3 Vone; temp _tmp_buf nullval;
+           gvar ___stringlit_1 ep; temp _out octx; temp _in ictx)
+    SEP (FRZL FR1;
+         data_at Tsh (Tstruct _env_md_ctx_st noattr) (t, (md, (nullval, nullval))) ictx; 
+         data_at_ Tsh tp md;
+         EVP_MD_NNnode tsh (*tvals*)(tpp, (mds, (flags, (ini, (upd, (fin, (blsize, Vint ctxsz))))))) t)).
+  { clear H. 
+    apply denote_tc_test_eq_split; try apply valid_pointer_null.
+    apply sepcon_valid_pointer1. apply sepcon_valid_pointer2. apply data_at_valid_ptr; [intuition | omega ]. }
+  { clear H. forward. 
+    unfold EVP_MD_NNnode; Intros. rename H into TSH.
+    (*destruct tvals as [tpp [mds [flags [ini [upd [fin [blsize ctxsize]]]]]]]; simpl in *; subst.*)
+    forward. forward. unfold EVP_MD_NNnode; entailer!. simpl. rewrite SZ2; trivial. }
+  { subst md; contradiction. }
+  thaw FR1.
+  forward_if (
+    PROP ( )
+    LOCAL (gvar ___stringlit_1 ep; temp _out octx; temp _in ictx)
+    SEP (EVP_MD_NNnode dsh dvals d; ERR ep;
+         data_at Tsh (Tstruct _env_md_ctx_st noattr) (t, (md, (nullval, nullval))) ictx;
+         data_at_ Tsh tp md; EVP_MD_NNnode tsh (*tvals*)(tpp, (mds, (flags, (ini, (upd, (fin, (blsize, Vint ctxsz))))))) t;
+         EX m :_, (!!(malloc_compatible (Int.unsigned ctxsz) m) 
+             && data_at Tsh (Tstruct _env_md_ctx_st noattr) (t, (m, (nullval, nullval))) octx * 
+                data_at_ Tsh tp m)));
+  [ clear H | inv H | ].
+  { forward_if (
+    PROP ( )
+    LOCAL (gvar ___stringlit_1 ep; temp _out octx; temp _in ictx)
+    SEP (EVP_MD_NNnode dsh dvals d; ERR ep;
+         data_at Tsh (Tstruct _env_md_ctx_st noattr) (t, (md, (nullval, nullval))) ictx;
+         data_at_ Tsh tp md; EVP_MD_NNnode tsh (*tvals*)(tpp, (mds, (flags, (ini, (upd, (fin, (blsize, Vint ctxsz))))))) t;
+         EX m :_, (!!(malloc_compatible (Int.unsigned ctxsz) m) 
+             && data_at Tsh (Tstruct _env_md_ctx_st noattr) (t, (m, (nullval, nullval))) octx * 
+                memory_block Tsh (Int.unsigned ctxsz) m))).
+    { contradiction. }
+    { clear H. forward. unfold EVP_MD_NNnode at 2; Intros. rename H into TSH.
+      (*destruct tvals as [tpp [mds [flags [ini [upd [fin [blsize ctxsize]]]]]]]; simpl in *; subst.*)
+      forward.
+      forward_call (Int.unsigned ctxsz).
+      { simpl; rewrite Int.repr_unsigned; entailer!. }
+      Intros m; forward. forward.
+      apply semax_orp_SEPx; Intros.
+      + (*m=Null*)
+        subst; simpl.
+        forward_if ( PROP (False) LOCAL () SEP ()).
+        - clear H.
+          forward_call (Vint (Int.repr 29), Vint (Int.repr 0), Vint (Int.or (Int.repr 1) (Int.repr 64)),
+                 ep, Vint (Int.repr 142)).
+          forward. Exists nullval. entailer!. unfold MDCTXFinished, EVP_MD_NNnode.
+          Exists md tp; unfold EVP_MD_CTX_NNnode; entailer!.
+          apply orp_right1. unfold MDCTXInitializedDigestSet. entailer!.
+        - inv H.
+        - intros. unfold POSTCONDITION, abbreviate, overridePost; clear POSTCONDITION.
+          old_go_lower. clear H. destruct ek; simpl; normalize. 
+      + (*m<>null*)
+        rename H into M. 
+        rewrite memory_block_isptr; Intros.
+        rewrite sem_cast_neutral_ptr; simpl; trivial.
+        forward_if (
+          PROP ( )
+          LOCAL (gvar ___stringlit_1 ep; temp _out octx; temp _in ictx)
+          SEP (memory_block Tsh (Int.unsigned ctxsz) m;
+               data_at Tsh (Tstruct _env_md_ctx_st noattr) (t, (m, (nullval, nullval))) octx; 
+               ERR ep; data_at_ Tsh tp md; EVP_MD_NNnode dsh dvals d;
+               data_at tsh (Tstruct _env_md_st noattr) (tpp, (mds, (flags, (ini, (upd, (fin, (blsize, Vint ctxsz))))))) t;
+               data_at Tsh (Tstruct _env_md_ctx_st noattr) (t, (md, (nullval, nullval))) ictx)).
+        - clear H.
+          apply denote_tc_test_eq_split; [ apply sepcon_valid_pointer1 | apply valid_pointer_null].
+          apply sepcon_valid_pointer1. apply sepcon_valid_pointer1. apply sepcon_valid_pointer1.
+          apply sepcon_valid_pointer1. apply sepcon_valid_pointer1. apply memory_block_valid_ptr. intuition. omega.
+        - destruct m; try contradiction. simpl in H. inv H.
+        - clear H. forward. entailer!.
+        - intros. unfold POSTCONDITION, abbreviate, overridePost; clear POSTCONDITION.
+          old_go_lower. clear H. destruct ek; simpl; normalize. entailer!.
+          Exists m; entailer!. unfold EVP_MD_NNnode; entailer!. }
+    Intros m. rename H into M. forward. forward. forward.
+    unfold EVP_MD_NNnode; Intros. rename H into TSH. 
+    (*destruct tvals as [tpp [mds [flags [ini [upd [fin [blsize ctxsize]]]]]]]; simpl in *; subst.*)
+    forward.
+(*    replace_SEP 1 (data_at Tsh tp (default_val tp) md) by entailer!.*)
+    replace_SEP 3 (data_at Tsh tp (default_val tp) md) by entailer!.
+    forward_call ((Tsh,Tsh),m, md, Int.unsigned ctxsz, Build_REPTYPE tp (default_val tp)).
+         { rewrite Int.repr_unsigned. simpl. apply prop_right; trivial. }
+         { simpl. cancel. }
+         { simpl in *; split; trivial. intuition. split; trivial.
+           split. apply Int.unsigned_range_2. rewrite SZ3; trivial. }
+    go_lower. normalize. Exists m; unfold EVP_MD_NNnode; normalize.
+    apply andp_right; [ apply prop_right; repeat split; trivial | cancel]. }
+  Intros m. rename H into M. forward. forward. forward. 
+  forward_if (
+    PROP ( )
+    LOCAL (temp _t'5 (Vint (Int.repr 0)); gvar ___stringlit_1 ep; temp _out octx; temp _in ictx)
+    SEP (EVP_MD_NNnode dsh dvals d; ERR ep;
+         data_at Tsh (Tstruct _env_md_ctx_st noattr) (t, (md, (nullval, nullval))) ictx;
+         data_at_ Tsh tp md; EVP_MD_NNnode tsh (*tvals*)(tpp, (mds, (flags, (ini, (upd, (fin, (blsize, Vint ctxsz))))))) t;
+         data_at Tsh (Tstruct _env_md_ctx_st noattr) (t, (m, (nullval, Vint Int.zero))) octx; 
+         data_at_ Tsh tp m)).
+  { contradiction. }
+  { clear H. forward. entailer!. }
+  forward_if (
+    PROP ( )
+    LOCAL (gvar ___stringlit_1 ep; temp _out octx; temp _in ictx)
+    SEP (EVP_MD_NNnode dsh dvals d; ERR ep;
+         data_at Tsh (Tstruct _env_md_ctx_st noattr) (t, (md, (nullval, nullval))) ictx;
+         data_at_ Tsh tp md; EVP_MD_NNnode tsh (*tvals*)(tpp, (mds, (flags, (ini, (upd, (fin, (blsize, Vint ctxsz))))))) t;
+         data_at Tsh (Tstruct _env_md_ctx_st noattr) (t, (m, (nullval, Vint Int.zero))) octx; 
+         data_at_ Tsh tp m)).
+  { contradiction. }
+  { clear H. forward. entailer!. }
+  forward. Exists Vone; unfold MDCTXFinished; entailer!.
+  Exists md tp. unfold EVP_MD_CTX_NNnode; entailer!.
+  apply orp_right2. Exists m tp; entailer!.
+Time Qed.
+
+Lemma body_EVP_MD_CTX_copy_ex_FinishedEQ: semax_body Vprog Gprog_copy_ex f_EVP_MD_CTX_copy_ex EVP_MD_CTX_copy_ex_SPEC_Finished_EQ.
+Proof. 
+  start_function. rename H into SZ. rename H0 into SZ1. forward.
+  rewrite MDCTXFinished_isptr' with (p:=ictx); Intros.
+  rewrite MDCTXFinished_isptr' with (p:=octx); Intros.
+  rewrite EVP_MD_NNnode_isptr'; Intros.
+  forward_if (
+    PROP ( )
+     LOCAL (temp _t'1 Vzero; temp _tmp_buf (Vint (Int.repr 0));
+            gvar ___stringlit_1 ep; temp _out octx; temp _in ictx)
+     SEP (ERR ep; MDCTXFinished nid ctxsz t octx; MDCTXFinished nid ctxsz t ictx; EVP_MD_NNnode tsh vals t)).
+  { clear H; 
+    apply denote_tc_test_eq_split; try apply valid_pointer_null.
+    apply sepcon_valid_pointer1. apply sepcon_valid_pointer2. apply MDCTXFinished_valid_ptr. }
+  { subst; contradiction. } 
+  { clear H. unfold MDCTXFinished, EVP_MD_CTX_NNnode. Intros md' tp' md tp.
+    unfold EVP_MD_NNnode; Intros.
+    forward. forward. entailer!.
+    + destruct t; try contradiction; simpl; trivial.
+    + unfold MDCTXFinished, EVP_MD_NNnode, EVP_MD_CTX_NNnode.
+      Exists md' tp' md tp; entailer!. }
+  forward_if (
+    PROP ( )
+    LOCAL (temp _tmp_buf (Vint (Int.repr 0));
+           gvar ___stringlit_1 ep; temp _out octx; temp _in ictx)
+    SEP (ERR ep; MDCTXFinished nid ctxsz t octx; MDCTXFinished nid ctxsz t ictx;
+         EVP_MD_NNnode tsh vals t)).
+  { elim H; trivial. }
+  { clear H; forward; entailer!. }
+  unfold MDCTXFinished, EVP_MD_CTX_NNnode. Intros md' tp' md tp.
+  rewrite H0 in H2; inv H2. clear H3.
+  rename H into SZ2. rename H0 into HTP. rename H1 into SZ3.
+  rewrite data_at__isptr with (p:=md); Intros.
+  rewrite data_at__isptr with (p:=md'); Intros.
+  forward. forward.
+  forward_if (
+    PROP ( )
+    LOCAL (temp _tmp_buf md'; gvar ___stringlit_1 ep;
+           temp _out octx; temp _in ictx)
+    SEP (ERR ep; EVP_MD_NNnode tsh vals t;
+         data_at Tsh (Tstruct _env_md_ctx_st noattr) (t, (nullval, (nullval, nullval))) octx;
+         data_at Tsh (Tstruct _env_md_ctx_st noattr) (t, (md, (nullval, nullval))) ictx;
+         data_at_ Tsh tp md; data_at_ Tsh tp md')).
+  { clear H.
+    apply denote_tc_test_eq_split; 
+    apply sepcon_valid_pointer2; apply EVP_MD_NNnode_validptr. }
+  { clear H. forward. forward. entailer!. }
+  { apply ptr_comp_Ceq_f in H; trivial; simpl in H. elim H; trivial. }
+  forward_call (octx, ClInitializedDigestSet t tsh vals).
+  { simpl. Exists ctxsz; unfold MDCTXInitializedDigestSet; entailer!. }
+  forward. simpl; unfold MDCTXInitialized; Intros. forward.
+  simpl. rewrite sem_cast_neutral_ptr; simpl; trivial.
+  forward.
+  forward_if (
+    PROP ( )
+    LOCAL (temp _t'3 Vone; temp _tmp_buf md';
+           gvar ___stringlit_1 ep; temp _out octx; temp _in ictx)
+    SEP (data_at Tsh (Tstruct _env_md_ctx_st noattr) (t, (nullval, (nullval, nullval))) octx; 
+         ERR ep; data_at_ Tsh tp md; EVP_MD_NNnode tsh vals t; data_at_ Tsh tp md';
+         data_at Tsh (Tstruct _env_md_ctx_st noattr) (t, (md, (nullval, nullval))) ictx)).
+  { clear H. 
+    apply denote_tc_test_eq_split; try apply valid_pointer_null.
+    apply sepcon_valid_pointer1. apply sepcon_valid_pointer2. apply data_at_valid_ptr; [intuition | omega ]. }
+  { clear H. forward. 
+    unfold EVP_MD_NNnode; Intros. rename H into TSH.
+    destruct vals as [tpp [mds [flags [ini [upd [fin [blsize ctxsize]]]]]]]; simpl in *; subst.
+    forward. forward. unfold EVP_MD_NNnode; entailer!. simpl. rewrite SZ2; trivial. }
+  { subst md; contradiction. }
+  forward_if (
+    PROP ( )
+    LOCAL (gvar ___stringlit_1 ep; temp _out octx; temp _in ictx)
+    SEP (ERR ep; data_at_ Tsh tp md; EVP_MD_NNnode tsh vals t;
+         data_at Tsh (Tstruct _env_md_ctx_st noattr) (t, (md', (nullval, nullval))) octx;
+         data_at Tsh (Tstruct _env_md_ctx_st noattr) (t, (md, (nullval, nullval))) ictx; 
+         data_at_ Tsh tp md'));
+  [ clear H | inv H | ].
+  { forward_if (
+    PROP ( )
+    LOCAL (gvar ___stringlit_1 ep; temp _out octx; temp _in ictx)
+    SEP (ERR ep; data_at_ Tsh tp md; EVP_MD_NNnode tsh vals t;
+         data_at Tsh (Tstruct _env_md_ctx_st noattr) (t, (md', (nullval, nullval))) octx;
+         data_at_ Tsh tp md';
+         data_at Tsh (Tstruct _env_md_ctx_st noattr) (t, (md, (nullval, nullval))) ictx)).
+    { clear H. apply denote_tc_test_eq_split; [ apply sepcon_valid_pointer1 | apply valid_pointer_null].
+      apply sepcon_valid_pointer2; apply data_at_valid_ptr; intuition. }
+    { clear H. forward. entailer!. cancel. } 
+    { subst; contradiction. }
+    forward. forward. forward. 
+    unfold EVP_MD_NNnode; Intros. rename H into TSH.
+    destruct vals as [tpp [mds [flags [ini [upd [fin [blsize ctxsize]]]]]]]; simpl in *; subst.
+    forward.
+    replace_SEP 4 (memory_block Tsh (Int.unsigned ctxsz) md').
+    { rewrite <- SZ3. entailer!. 
+      eapply derives_trans; [ apply data_at_memory_block | cancel]. }
+    replace_SEP 1 (data_at Tsh tp (default_val tp) md) by entailer!.
+    forward_call ((Tsh,Tsh),md', md, Int.unsigned ctxsz, Build_REPTYPE tp (default_val tp)).
+         { rewrite Int.repr_unsigned. simpl. apply prop_right; trivial. }
+         { simpl. cancel. }
+         { simpl in *; split; trivial. intuition. split; trivial.
+           split. apply Int.unsigned_range_2. rewrite SZ3; trivial. }
+    entailer!. unfold EVP_MD_NNnode; entailer!. }
+
+  forward. forward. forward. 
+  forward_if (
+    PROP ( )
+    LOCAL (temp _t'5 (Vint (Int.repr 0)); gvar ___stringlit_1 ep; temp _out octx; temp _in ictx)
+    SEP (ERR ep; data_at_ Tsh tp md; EVP_MD_NNnode tsh vals t;
+         data_at Tsh (Tstruct _env_md_ctx_st noattr) (t, (md', (nullval, Vint Int.zero))) octx;
+         data_at_ Tsh tp md';
+         data_at Tsh (Tstruct _env_md_ctx_st noattr) (t, (md, (nullval, nullval))) ictx)).
+  { contradiction. }
+  { clear H. forward. entailer!. }
+  forward_if (
+    PROP ( )
+    LOCAL (gvar ___stringlit_1 ep; temp _out octx; temp _in ictx)
+    SEP (ERR ep; data_at_ Tsh tp md; EVP_MD_NNnode tsh vals t;
+         data_at Tsh (Tstruct _env_md_ctx_st noattr) (t, (md', (nullval, Vint Int.zero))) octx;
+         data_at_ Tsh tp md';
+         data_at Tsh (Tstruct _env_md_ctx_st noattr) (t, (md, (nullval, nullval))) ictx)).
+  { contradiction. }
+  { clear H. forward. entailer!. }
+  forward. cancel. unfold MDCTXFinished, EVP_MD_CTX_NNnode.
+  Exists md md' tp tp; entailer!.
+Time Qed.
+
+(*Also supports Hashed octx, since Hashed octx |-- Finished octx.
+  Allocation is performed, and result may be Vone or Vnull*)
+Definition EVP_MD_CTX_copy_ex_SPEC_Hashed_NEQ := DECLARE _EVP_MD_CTX_copy_ex
+  WITH ep: val, octx:val, ictx:val,
+       nid:int, ctxsz:int , data:list int, sh:share * share, vals:_, t:val,
+       nid':int, ctxsz':int, d:val
+  PRE [ _out OF (tptr (Tstruct _env_md_ctx_st noattr)),
+        _in OF (tptr (Tstruct _env_md_ctx_st noattr)) ]
+      PROP (get_ctxsize (snd vals) = Vint ctxsz' /\ get_type (snd vals) = Vint nid';
+            get_ctxsize (fst vals) = Vint ctxsz; 4 <= Int.unsigned ctxsz <= Int.max_unsigned; d<>t)
+      LOCAL (gvar ___stringlit_1 ep; temp _out octx; temp _in ictx)
+      SEP (ERR ep; MDCTXFinished nid' ctxsz' d octx; 
+           MDCTXHashed nid ctxsz (map Int.unsigned data) t ictx;
+           EVP_MD_NNnode (fst sh) (fst vals) t; EVP_MD_NNnode (snd sh) (snd vals) d)
+  POST [ tint] EX rv:_,
+       PROP ()
+       LOCAL (temp ret_temp rv)
+       SEP (ERR ep; MDCTXHashed nid ctxsz (map Int.unsigned data) t ictx; 
+            EVP_MD_NNnode (fst sh) (fst vals) t; EVP_MD_NNnode (snd sh) (snd vals) d;
+            (!!(rv=nullval) && MDCTXInitializedDigestSet t octx) 
+            || (!!(rv=Vone) && MDCTXHashed nid ctxsz (map Int.unsigned data) t octx)).
+
+(*Also supports Hashed octx, since Hashed octx |-- Finished octx.
+  No allocation is performed, and result value is always Vone*)
+Definition EVP_MD_CTX_copy_ex_SPEC_Hashed_EQ := DECLARE _EVP_MD_CTX_copy_ex
+  WITH ep: val, octx:val, ictx:val,
+       nid:int, ctxsz:int, data:list int, tsh:share, vals:_, t:val
+  PRE [ _out OF (tptr (Tstruct _env_md_ctx_st noattr)),
+        _in OF (tptr (Tstruct _env_md_ctx_st noattr)) ]
+      PROP (get_ctxsize vals = Vint ctxsz; 4 <= Int.unsigned ctxsz <= Int.max_unsigned)
+      LOCAL (gvar ___stringlit_1 ep; temp _out octx; temp _in ictx)
+      SEP (ERR ep; MDCTXFinished nid ctxsz t octx; 
+           MDCTXHashed nid ctxsz (map Int.unsigned data) t ictx;
+           EVP_MD_NNnode tsh vals t)
+  POST [ tint] 
+       PROP ()
+       LOCAL (temp ret_temp Vone)
+       SEP (ERR ep; MDCTXHashed nid ctxsz (map Int.unsigned data) t ictx; EVP_MD_NNnode tsh vals t;
+            MDCTXHashed nid ctxsz (map Int.unsigned data) t octx).
+
+
+Lemma body_EVP_MD_CTX_copy_ex_Hashed_NEQ: semax_body Vprog Gprog_copy_ex f_EVP_MD_CTX_copy_ex EVP_MD_CTX_copy_ex_SPEC_Hashed_NEQ.
+Proof. 
+  start_function. destruct H as [SZ' NID'].
+  rename H0 into SZ. rename H1 into SZ1. rename H2 into DT. forward.
+  rewrite MDCTXHashed_isptr'; Intros.
+  rewrite MDCTXFinished_isptr'; Intros.
+  rewrite EVP_MD_NNnode_isptr' with (p:= t); Intros.
+  rewrite EVP_MD_NNnode_isptr' with (p:= d); Intros.
+  destruct sh as [tsh dsh]. destruct vals as [tvals dvals]; simpl in *.
+  destruct tvals as [tpp [mds [flags [ini [upd [fin [blsize ctxsize]]]]]]]; simpl in *; subst.
+  freeze [0;1;4] FR1.
+  forward_if (
+    PROP ( )
+     LOCAL (temp _t'1 Vzero; temp _tmp_buf (Vint (Int.repr 0));
+            gvar ___stringlit_1 ep; temp _out octx; temp _in ictx)
+     SEP (FRZL FR1; MDCTXHashed nid ctxsz (map Int.unsigned data) t ictx;
+          EVP_MD_NNnode tsh (*tvals*)(tpp, (mds, (flags, (ini, (upd, (fin, (blsize, Vint ctxsz))))))) t)).
+  { clear H; 
+    apply denote_tc_test_eq_split; try apply valid_pointer_null.
+    apply sepcon_valid_pointer1. 
+    apply sepcon_valid_pointer2. apply MDCTXHashed_valid_ptr. }
+  { subst; contradiction. } 
+  { clear H. unfold MDCTXHashed. unfold EVP_MD_CTX_NNnode. Intros md tp v.
+    unfold EVP_MD_NNnode; Intros.
+    forward. forward. entailer!.
+    + destruct t; try contradiction; simpl; trivial.
+    + unfold MDCTXHashed, EVP_MD_NNnode, EVP_MD_CTX_NNnode. Exists md tp v; entailer!. }
+  forward_if (
+    PROP ( )
+    LOCAL (temp _tmp_buf (Vint (Int.repr 0));
+           gvar ___stringlit_1 ep; temp _out octx; temp _in ictx)
+    SEP (FRZL FR1; MDCTXHashed nid ctxsz (map Int.unsigned data) t ictx;
+         EVP_MD_NNnode tsh (*tvals*)(tpp, (mds, (flags, (ini, (upd, (fin, (blsize, Vint ctxsz))))))) t)).
+  { elim H; trivial. }
+  { clear H; forward; entailer!. }
+  thaw FR1.
+      unfold MDCTXFinished, MDCTXHashed, EVP_MD_CTX_NNnode. Intros md' tp' md tp v.
+      rename H into SZ2'. rename H0 into TP'. rename H1 into SZ3'. (* rename H2 into V'.*)
+      rename H2 into SZ2. rename H3 into TP. rename H4 into SZ3. rename H5 into V.
+      rewrite data_at_isptr with (p:=md); Intros.
+      rewrite data_at__isptr with (p:=md'); Intros.
+      forward. forward.
+      forward_if (
+        PROP ( )
+        LOCAL (temp _tmp_buf (Vint (Int.repr 0)); gvar ___stringlit_1 ep;
+               temp _out octx; temp _in ictx)
+        SEP (ERR ep;
+             data_at Tsh (Tstruct _env_md_ctx_st noattr) (d, (md', (nullval, nullval))) octx;
+             data_at_ Tsh tp' md'; EVP_MD_NNnode dsh dvals d;
+             data_at Tsh (Tstruct _env_md_ctx_st noattr) (t, (md, (nullval, nullval))) ictx;
+             data_at Tsh tp v md; EVP_MD_NNnode tsh (*tvals*)(tpp, (mds, (flags, (ini, (upd, (fin, (blsize, Vint ctxsz))))))) t)).
+      { clear H.
+        apply denote_tc_test_eq_split; 
+        [ apply sepcon_valid_pointer1 | apply sepcon_valid_pointer2; apply EVP_MD_NNnode_validptr ].
+        apply sepcon_valid_pointer1; apply sepcon_valid_pointer1. apply sepcon_valid_pointer2; apply EVP_MD_NNnode_validptr. }
+      { apply ptr_comp_Ceq_t in H; trivial; simpl in H. congruence. }
+      { forward; entailer!. }
+  gather_SEP 1 2.
+  replace_SEP 0 (MDCTXConfigured nid' ctxsz' d octx || MDCTXFinished nid' ctxsz' d octx).
+  { unfold MDCTXFinished; entailer!. apply orp_right2. Exists md' tp'; entailer!. }
+  forward_call (octx, ClConfiguredOrFinished dsh dvals d).
+  { simpl. Exists nid' ctxsz'; entailer!. }
+  simpl. normalize.
+  rewrite data_at_isptr with (p:=md); Intros.
+  forward. simpl; unfold MDCTXInitialized; Intros. forward.
+  simpl. rewrite sem_cast_neutral_ptr; simpl; trivial.
+  forward. freeze [0;1;2] FR1.
+  forward_if (
+    PROP ( )
+    LOCAL (temp _t'3 Vone; temp _tmp_buf nullval;
+           gvar ___stringlit_1 ep; temp _out octx; temp _in ictx)
+    SEP (FRZL FR1;
+         data_at Tsh (Tstruct _env_md_ctx_st noattr) (t, (md, (nullval, nullval))) ictx; data_at Tsh tp v md;
+         EVP_MD_NNnode tsh (*tvals*)(tpp, (mds, (flags, (ini, (upd, (fin, (blsize, Vint ctxsz))))))) t)).
+  { clear H. 
+    apply denote_tc_test_eq_split; try apply valid_pointer_null.
+    apply sepcon_valid_pointer1. apply sepcon_valid_pointer2. apply data_at_valid_ptr; [intuition | omega ]. }
+  { clear H. forward. 
+    unfold EVP_MD_NNnode; Intros. rename H into TSH.
+    (*destruct tvals as [tpp [mds [flags [ini [upd [fin [blsize ctxsize]]]]]]]; simpl in *; subst.*)
+    forward. forward. unfold EVP_MD_NNnode; entailer!. simpl. rewrite SZ2; trivial. }
+  { subst md; contradiction. }
+  thaw FR1.
+  forward_if (
+    PROP ( )
+    LOCAL (gvar ___stringlit_1 ep; temp _out octx; temp _in ictx)
+    SEP (EVP_MD_NNnode dsh dvals d; ERR ep;
+         data_at Tsh (Tstruct _env_md_ctx_st noattr) (t, (md, (nullval, nullval))) ictx;
+         data_at Tsh tp v md; EVP_MD_NNnode tsh (*tvals*)(tpp, (mds, (flags, (ini, (upd, (fin, (blsize, Vint ctxsz))))))) t;
+         EX m :_, (!!(malloc_compatible (Int.unsigned ctxsz) m) 
+             && data_at Tsh (Tstruct _env_md_ctx_st noattr) (t, (m, (nullval, nullval))) octx * 
+                data_at Tsh tp v m)));
+  [ clear H | inv H | ].
+  { forward_if (
+    PROP ( )
+    LOCAL (gvar ___stringlit_1 ep; temp _out octx; temp _in ictx)
+    SEP (EVP_MD_NNnode dsh dvals d; ERR ep;
+         data_at Tsh (Tstruct _env_md_ctx_st noattr) (t, (md, (nullval, nullval))) ictx;
+         data_at Tsh tp v md; EVP_MD_NNnode tsh (*tvals*)(tpp, (mds, (flags, (ini, (upd, (fin, (blsize, Vint ctxsz))))))) t;
+         EX m :_, (!!(malloc_compatible (Int.unsigned ctxsz) m) 
+             && data_at Tsh (Tstruct _env_md_ctx_st noattr) (t, (m, (nullval, nullval))) octx * 
+                memory_block Tsh (Int.unsigned ctxsz) m))).
+    { contradiction. }
+    { clear H. forward. unfold EVP_MD_NNnode at 2; Intros. rename H into TSH.
+      (*destruct tvals as [tpp [mds [flags [ini [upd [fin [blsize ctxsize]]]]]]]; simpl in *; subst.*)
+      forward.
+      forward_call (Int.unsigned ctxsz).
+      { simpl; rewrite Int.repr_unsigned; entailer!. }
+      Intros m; forward. forward.
+      apply semax_orp_SEPx; Intros.
+      + (*m=Null*)
+        subst; simpl.
+        forward_if ( PROP (False) LOCAL () SEP ()).
+        - clear H.
+          forward_call (Vint (Int.repr 29), Vint (Int.repr 0), Vint (Int.or (Int.repr 1) (Int.repr 64)),
+                 ep, Vint (Int.repr 142)).
+          forward. Exists nullval. entailer!. unfold MDCTXHashed, EVP_MD_NNnode.
+          Exists md tp; unfold EVP_MD_CTX_NNnode; entailer!.
+          Exists v. entailer!. 
+          apply orp_right1. unfold MDCTXInitializedDigestSet. entailer!.
+        - inv H.
+        - intros. unfold POSTCONDITION, abbreviate, overridePost; clear POSTCONDITION.
+          old_go_lower. clear H. destruct ek; simpl; normalize. 
+      + (*m<>null*)
+        rename H into M. 
+        rewrite memory_block_isptr; Intros.
+        rewrite sem_cast_neutral_ptr; simpl; trivial.
+        forward_if (
+          PROP ( )
+          LOCAL (gvar ___stringlit_1 ep; temp _out octx; temp _in ictx)
+          SEP (memory_block Tsh (Int.unsigned ctxsz) m;
+               data_at Tsh (Tstruct _env_md_ctx_st noattr) (t, (m, (nullval, nullval))) octx; 
+               ERR ep; data_at Tsh tp v md; EVP_MD_NNnode dsh dvals d;
+               data_at tsh (Tstruct _env_md_st noattr) (tpp, (mds, (flags, (ini, (upd, (fin, (blsize, Vint ctxsz))))))) t;
+               data_at Tsh (Tstruct _env_md_ctx_st noattr) (t, (md, (nullval, nullval))) ictx)).
+        - clear H.
+          apply denote_tc_test_eq_split; [ apply sepcon_valid_pointer1 | apply valid_pointer_null].
+          apply sepcon_valid_pointer1. apply sepcon_valid_pointer1. apply sepcon_valid_pointer1.
+          apply sepcon_valid_pointer1. apply sepcon_valid_pointer1. apply memory_block_valid_ptr. intuition. omega.
+        - destruct m; try contradiction. simpl in H. inv H.
+        - clear H. forward. entailer!.
+        - intros. unfold POSTCONDITION, abbreviate, overridePost; clear POSTCONDITION.
+          old_go_lower. clear H. destruct ek; simpl; normalize. entailer!.
+          Exists m; entailer!. unfold EVP_MD_NNnode; entailer!. }
+    Intros m. rename H into M. forward. forward. forward.
+    unfold EVP_MD_NNnode; Intros. rename H into TSH. 
+    (*destruct tvals as [tpp [mds [flags [ini [upd [fin [blsize ctxsize]]]]]]]; simpl in *; subst.*)
+    forward. 
+(*    replace_SEP 1 (data_at Tsh tp (default_val tp) md) by entailer!.*)
+    forward_call ((Tsh,Tsh),m, md, Int.unsigned ctxsz, Build_REPTYPE tp v).
+         { rewrite Int.repr_unsigned. simpl. apply prop_right; trivial. }
+         { simpl. cancel. }
+         { simpl in *; split; trivial. intuition. split; trivial.
+           split. apply Int.unsigned_range_2. rewrite SZ3; trivial. }
+    go_lower. normalize. Exists m; unfold EVP_MD_NNnode; normalize.
+    apply andp_right; [ apply prop_right; repeat split; trivial | cancel]. }
+  Intros m. rename H into M. forward. forward. forward. 
+  forward_if (
+    PROP ( )
+    LOCAL (temp _t'5 (Vint (Int.repr 0)); gvar ___stringlit_1 ep; temp _out octx; temp _in ictx)
+    SEP (EVP_MD_NNnode dsh dvals d; ERR ep;
+         data_at Tsh (Tstruct _env_md_ctx_st noattr) (t, (md, (nullval, nullval))) ictx;
+         data_at Tsh tp v md; EVP_MD_NNnode tsh (*tvals*)(tpp, (mds, (flags, (ini, (upd, (fin, (blsize, Vint ctxsz))))))) t;
+         data_at Tsh (Tstruct _env_md_ctx_st noattr) (t, (m, (nullval, Vint Int.zero))) octx; 
+         data_at Tsh tp v m)).
+  { contradiction. }
+  { clear H. forward. entailer!. }
+  forward_if (
+    PROP ( )
+    LOCAL (gvar ___stringlit_1 ep; temp _out octx; temp _in ictx)
+    SEP (EVP_MD_NNnode dsh dvals d; ERR ep;
+         data_at Tsh (Tstruct _env_md_ctx_st noattr) (t, (md, (nullval, nullval))) ictx;
+         data_at Tsh tp v md; EVP_MD_NNnode tsh (*tvals*)(tpp, (mds, (flags, (ini, (upd, (fin, (blsize, Vint ctxsz))))))) t;
+         data_at Tsh (Tstruct _env_md_ctx_st noattr) (t, (m, (nullval, Vint Int.zero))) octx; 
+         data_at Tsh tp v m)).
+  { contradiction. }
+  { clear H. forward. entailer!. }
+  forward. Exists Vone; unfold MDCTXHashed; entailer!.
+  Exists md tp v. unfold EVP_MD_CTX_NNnode; entailer!.
+  apply orp_right2. Exists m tp v; entailer!.
+Time Qed.
+
+Lemma body_EVP_MD_CTX_copy_ex_HashedEQ: semax_body Vprog Gprog_copy_ex f_EVP_MD_CTX_copy_ex EVP_MD_CTX_copy_ex_SPEC_Hashed_EQ.
+Proof. 
+  start_function. rename H into SZ. rename H0 into SZ1. forward.
+  rewrite MDCTXHashed_isptr' with (p:=ictx); Intros.
+  rewrite MDCTXFinished_isptr' with (p:=octx); Intros.
+  rewrite EVP_MD_NNnode_isptr'; Intros.
+  forward_if (
+    PROP ( )
+     LOCAL (temp _t'1 Vzero; temp _tmp_buf (Vint (Int.repr 0));
+            gvar ___stringlit_1 ep; temp _out octx; temp _in ictx)
+     SEP (ERR ep; MDCTXFinished nid ctxsz t octx; MDCTXHashed nid ctxsz (map Int.unsigned data) t ictx; EVP_MD_NNnode tsh vals t)).
+  { clear H; 
+    apply denote_tc_test_eq_split; try apply valid_pointer_null.
+    apply sepcon_valid_pointer1. apply sepcon_valid_pointer2. apply MDCTXHashed_valid_ptr. }
+  { subst; contradiction. } 
+  { clear H. unfold MDCTXHashed, EVP_MD_CTX_NNnode. Intros md tp v.
+    unfold EVP_MD_NNnode; Intros.
+    forward. forward. entailer!.
+    + destruct t; try contradiction; simpl; trivial.
+    + unfold MDCTXHashed, EVP_MD_NNnode, EVP_MD_CTX_NNnode. Exists md tp v; entailer!. }
+  forward_if (
+    PROP ( )
+    LOCAL (temp _tmp_buf (Vint (Int.repr 0));
+           gvar ___stringlit_1 ep; temp _out octx; temp _in ictx)
+    SEP (ERR ep; MDCTXFinished nid ctxsz t octx; MDCTXHashed nid ctxsz (map Int.unsigned data) t ictx;
+         EVP_MD_NNnode tsh vals t)).
+  { elim H; trivial. }
+  { clear H; forward; entailer!. }
+  unfold MDCTXFinished, MDCTXHashed, EVP_MD_CTX_NNnode. Intros md' tp' md tp v.
+  rewrite H0 in H2; inv H2. clear H3. rename H4 into V.
+  rename H into SZ2. rename H0 into HTP. rename H1 into SZ3.
+  rewrite data_at_isptr with (p:=md); Intros.
+  rewrite data_at__isptr with (p:=md'); Intros.
+  forward. forward.
+  forward_if (
+    PROP ( )
+    LOCAL (temp _tmp_buf md'; gvar ___stringlit_1 ep;
+           temp _out octx; temp _in ictx)
+    SEP (ERR ep; EVP_MD_NNnode tsh vals t;
+         data_at Tsh (Tstruct _env_md_ctx_st noattr) (t, (nullval, (nullval, nullval))) octx;
+         data_at Tsh (Tstruct _env_md_ctx_st noattr) (t, (md, (nullval, nullval))) ictx;
+         data_at Tsh tp v md; data_at_ Tsh tp md')).
+  { clear H.
+    apply denote_tc_test_eq_split; 
+    apply sepcon_valid_pointer2; apply EVP_MD_NNnode_validptr. }
+  { clear H. forward. forward. entailer!. }
+  { apply ptr_comp_Ceq_f in H; trivial; simpl in H. elim H; trivial. }
+  forward_call (octx, ClInitializedDigestSet t tsh vals).
+  { simpl. Exists ctxsz; unfold MDCTXInitializedDigestSet; entailer!. }
+  forward. simpl; unfold MDCTXInitialized; Intros. forward.
+  simpl. rewrite sem_cast_neutral_ptr; simpl; trivial.
+  forward.
+  forward_if (
+    PROP ( )
+    LOCAL (temp _t'3 Vone; temp _tmp_buf md';
+           gvar ___stringlit_1 ep; temp _out octx; temp _in ictx)
+    SEP (data_at Tsh (Tstruct _env_md_ctx_st noattr) (t, (nullval, (nullval, nullval))) octx; 
+         ERR ep; data_at Tsh tp v md; EVP_MD_NNnode tsh vals t; data_at_ Tsh tp md';
+         data_at Tsh (Tstruct _env_md_ctx_st noattr) (t, (md, (nullval, nullval))) ictx)).
+  { clear H. 
+    apply denote_tc_test_eq_split; try apply valid_pointer_null.
+    apply sepcon_valid_pointer1. apply sepcon_valid_pointer2. apply data_at_valid_ptr; [intuition | omega ]. }
+  { clear H. forward. 
+    unfold EVP_MD_NNnode; Intros. rename H into TSH.
+    destruct vals as [tpp [mds [flags [ini [upd [fin [blsize ctxsize]]]]]]]; simpl in *; subst.
+    forward. forward. unfold EVP_MD_NNnode; entailer!. simpl. rewrite SZ2; trivial. }
+  { subst md; contradiction. }
+  forward_if (
+    PROP ( )
+    LOCAL (gvar ___stringlit_1 ep; temp _out octx; temp _in ictx)
+    SEP (ERR ep; data_at Tsh tp v md; EVP_MD_NNnode tsh vals t;
+         data_at Tsh (Tstruct _env_md_ctx_st noattr) (t, (md', (nullval, nullval))) octx;
+         data_at Tsh (Tstruct _env_md_ctx_st noattr) (t, (md, (nullval, nullval))) ictx; 
+         data_at Tsh tp v md'));
+  [ clear H | inv H | ].
+  { forward_if (
+    PROP ( )
+    LOCAL (gvar ___stringlit_1 ep; temp _out octx; temp _in ictx)
+    SEP (ERR ep; data_at Tsh tp v md; EVP_MD_NNnode tsh vals t;
+         data_at Tsh (Tstruct _env_md_ctx_st noattr) (t, (md', (nullval, nullval))) octx;
+         data_at_ Tsh tp md';
+         data_at Tsh (Tstruct _env_md_ctx_st noattr) (t, (md, (nullval, nullval))) ictx)).
+    { clear H. apply denote_tc_test_eq_split; [ apply sepcon_valid_pointer1 | apply valid_pointer_null].
+      apply sepcon_valid_pointer2; apply data_at_valid_ptr; intuition. }
+    { clear H. forward. entailer!. cancel. } 
+    { subst; contradiction. }
+    forward. forward. forward. 
+    unfold EVP_MD_NNnode; Intros. rename H into TSH.
+    destruct vals as [tpp [mds [flags [ini [upd [fin [blsize ctxsize]]]]]]]; simpl in *; subst.
+    forward.
+    replace_SEP 4 (memory_block Tsh (Int.unsigned ctxsz) md').
+    { rewrite <- SZ3. entailer!. 
+      eapply derives_trans; [ apply data_at_memory_block | cancel]. }
+    forward_call ((Tsh,Tsh),md', md,Int.unsigned ctxsz, Build_REPTYPE tp v). 
+         { rewrite Int.repr_unsigned; entailer!. }
+         { simpl. cancel. }
+         { simpl; split; trivial. intuition. split; trivial. 
+           split. apply Int.unsigned_range_2. rewrite SZ3; trivial. }
+    entailer!. unfold EVP_MD_NNnode; entailer!. }
+
+  forward. forward. forward. 
+  forward_if (
+    PROP ( )
+    LOCAL (temp _t'5 (Vint (Int.repr 0)); gvar ___stringlit_1 ep; temp _out octx; temp _in ictx)
+    SEP (ERR ep; data_at Tsh tp v md; EVP_MD_NNnode tsh vals t;
+         data_at Tsh (Tstruct _env_md_ctx_st noattr) (t, (md', (nullval, Vint Int.zero))) octx;
+         data_at Tsh tp v md';
+         data_at Tsh (Tstruct _env_md_ctx_st noattr) (t, (md, (nullval, nullval))) ictx)).
+  { contradiction. }
+  { clear H. forward. entailer!. }
+  forward_if (
+    PROP ( )
+    LOCAL (gvar ___stringlit_1 ep; temp _out octx; temp _in ictx)
+    SEP (ERR ep; data_at Tsh tp v md; EVP_MD_NNnode tsh vals t;
+         data_at Tsh (Tstruct _env_md_ctx_st noattr) (t, (md', (nullval, Vint Int.zero))) octx;
+         data_at Tsh tp v md';
+         data_at Tsh (Tstruct _env_md_ctx_st noattr) (t, (md, (nullval, nullval))) ictx)).
+  { contradiction. }
+  { clear H. forward. entailer!. }
+  forward. cancel. unfold MDCTXHashed, EVP_MD_CTX_NNnode.
+  Exists md md' tp v tp v; entailer!.
+Time Qed.
+
+End EVP_MD_CTX_Protocol.
+
+(*
 (*Raises PUTERROR, even before octx is inspected. It's odd that we're not allowed to copy initialized digests...*)
 Definition EVP_MD_CTX_copy_ex_SPEC_Initialized := DECLARE _EVP_MD_CTX_copy_ex
   WITH ep: val, octx:val, ictx:val
@@ -1611,6 +3389,39 @@ Definition EVP_MD_CTX_copy_ex_SPEC_Initialized := DECLARE _EVP_MD_CTX_copy_ex
        PROP ()
        LOCAL (temp ret_temp nullval)
        SEP (ERR ep; (*MDCTXInitialized octx;*) MDCTXInitialized ictx).
+
+Definition EVP_MD_CTX_copy_ex_SPEC_Hashed2 := DECLARE _EVP_MD_CTX_copy_ex
+  WITH ep: val, octx:val, ictx:val,
+       nid:int, ctxsz:int, data:list int, data':list int, tsh:share, vals:_, t:val
+  PRE [ _out OF (tptr (Tstruct _env_md_ctx_st noattr)),
+        _in OF (tptr (Tstruct _env_md_ctx_st noattr)) ]
+      PROP (get_ctxsize vals = Vint ctxsz; 4 <= Int.unsigned ctxsz <= Int.max_unsigned)
+      LOCAL (gvar ___stringlit_1 ep; temp _out octx; temp _in ictx)
+      SEP (ERR ep; MDCTXHashed nid ctxsz (map Int.unsigned data') t octx; 
+           MDCTXHashed nid ctxsz (map Int.unsigned data) t ictx;
+           EVP_MD_NNnode tsh vals t)
+  POST [ tint] EX rv:_,
+       PROP ()
+       LOCAL (temp ret_temp rv)
+       SEP (ERR ep; MDCTXHashed nid ctxsz (map Int.unsigned data) t ictx; EVP_MD_NNnode tsh vals t;
+            (!!(rv=nullval) && MDCTXInitializedDigestSet t octx) 
+            || (!!(rv=Vone) && MDCTXHashed nid ctxsz (map Int.unsigned data) t octx)(*; copyExPost case ictx octx rv*)).
+
+Definition EVP_MD_CTX_copy_ex_SPEC_Finished := DECLARE _EVP_MD_CTX_copy_ex
+  WITH ep: val, octx:val, ictx:val,
+       nid:int, ctxsz:int, tsh:share, vals:_, t:val
+  PRE [ _out OF (tptr (Tstruct _env_md_ctx_st noattr)),
+        _in OF (tptr (Tstruct _env_md_ctx_st noattr)) ]
+      PROP (get_ctxsize vals = Vint ctxsz; 4 <= Int.unsigned ctxsz <= Int.max_unsigned)
+      LOCAL (gvar ___stringlit_1 ep; temp _out octx; temp _in ictx)
+      SEP (ERR ep;MDCTXInitialized octx; MDCTXFinished nid ctxsz t ictx;
+           EVP_MD_NNnode tsh vals t)
+  POST [ tint] EX rv:_,
+       PROP ()
+       LOCAL (temp ret_temp rv)
+       SEP (ERR ep; MDCTXFinished nid ctxsz t ictx; EVP_MD_NNnode tsh vals t;
+            (!!(rv=nullval) && MDCTXInitializedDigestSet t octx) 
+            || (!!(rv=Vone) && MDCTXFinished nid ctxsz t octx)).
 
 Lemma body_EVP_MD_CTX_copy_exI: semax_body Vprog Gprog_copy_ex f_EVP_MD_CTX_copy_ex EVP_MD_CTX_copy_ex_SPEC_Initialized.
 Proof. 
@@ -1634,22 +3445,6 @@ Proof.
   { inv H. }
   normalize.
 Qed.
-
-Definition EVP_MD_CTX_copy_ex_SPEC_Hashed := DECLARE _EVP_MD_CTX_copy_ex
-  WITH ep: val, octx:val, ictx:val,
-       nid:int, ctxsz:int, data:list int, tsh:share, vals:_, t:val
-  PRE [ _out OF (tptr (Tstruct _env_md_ctx_st noattr)),
-        _in OF (tptr (Tstruct _env_md_ctx_st noattr)) ]
-      PROP (get_ctxsize vals = Vint ctxsz; 4 <= Int.unsigned ctxsz <= Int.max_unsigned)
-      LOCAL (gvar ___stringlit_1 ep; temp _out octx; temp _in ictx)
-      SEP (ERR ep;MDCTXInitialized octx; MDCTXHashed nid ctxsz (map Int.unsigned data) t ictx;
-           EVP_MD_NNnode tsh vals t)
-  POST [ tint] EX rv:_,
-       PROP ()
-       LOCAL (temp ret_temp rv)
-       SEP (ERR ep; MDCTXHashed nid ctxsz (map Int.unsigned data) t ictx; EVP_MD_NNnode tsh vals t;
-            (!!(rv=nullval) && MDCTXInitialized_MDSET t octx) 
-            || (!!(rv=Vone) && MDCTXHashed nid ctxsz (map Int.unsigned data) t octx)(*; copyExPost case ictx octx rv*)).
 
 Lemma body_EVP_MD_CTX_copy_exH: semax_body Vprog Gprog_copy_ex f_EVP_MD_CTX_copy_ex EVP_MD_CTX_copy_ex_SPEC_Hashed.
 Proof. 
@@ -1752,7 +3547,7 @@ Proof.
                  ep, Vint (Int.repr 142)).
           forward. Exists nullval. entailer!. unfold MDCTXHashed, EVP_MD_NNnode.
           Exists md tp v; unfold EVP_MD_CTX_NNnode; entailer!.
-          apply orp_right1. unfold MDCTXInitialized_MDSET. cancel.
+          apply orp_right1. unfold MDCTXInitializedDigestSet. cancel.
         - inv H.
         - intros. unfold POSTCONDITION, abbreviate, overridePost; clear POSTCONDITION.
           old_go_lower. clear H. destruct ek; simpl; normalize. 
@@ -1822,22 +3617,6 @@ Proof.
   Exists md tp v. unfold EVP_MD_CTX_NNnode; entailer!.
   apply orp_right2. Exists m tp v; entailer!.
 Time Qed.
-
-Definition EVP_MD_CTX_copy_ex_SPEC_Finished := DECLARE _EVP_MD_CTX_copy_ex
-  WITH ep: val, octx:val, ictx:val,
-       nid:int, ctxsz:int, tsh:share, vals:_, t:val
-  PRE [ _out OF (tptr (Tstruct _env_md_ctx_st noattr)),
-        _in OF (tptr (Tstruct _env_md_ctx_st noattr)) ]
-      PROP (get_ctxsize vals = Vint ctxsz; 4 <= Int.unsigned ctxsz <= Int.max_unsigned)
-      LOCAL (gvar ___stringlit_1 ep; temp _out octx; temp _in ictx)
-      SEP (ERR ep;MDCTXInitialized octx; MDCTXFinished nid ctxsz t ictx;
-           EVP_MD_NNnode tsh vals t)
-  POST [ tint] EX rv:_,
-       PROP ()
-       LOCAL (temp ret_temp rv)
-       SEP (ERR ep; MDCTXFinished nid ctxsz t ictx; EVP_MD_NNnode tsh vals t;
-            (!!(rv=nullval) && MDCTXInitialized_MDSET t octx) 
-            || (!!(rv=Vone) && MDCTXFinished nid ctxsz t octx)).
 
 Lemma body_EVP_MD_CTX_copy_exF: semax_body Vprog Gprog_copy_ex f_EVP_MD_CTX_copy_ex EVP_MD_CTX_copy_ex_SPEC_Finished.
 Proof. 
@@ -1940,7 +3719,7 @@ Proof.
                  ep, Vint (Int.repr 142)).
           forward. Exists nullval. entailer!. unfold MDCTXFinished, EVP_MD_NNnode.
           Exists md tp; unfold EVP_MD_CTX_NNnode; entailer!.
-          apply orp_right1. unfold MDCTXInitialized_MDSET. cancel.
+          apply orp_right1. unfold MDCTXInitializedDigestSet. cancel.
         - inv H.
         - intros. unfold POSTCONDITION, abbreviate, overridePost; clear POSTCONDITION.
           old_go_lower. clear H. destruct ek; simpl; normalize. 
@@ -4510,4 +6289,4 @@ Definition EVP_MD_CTX_rep (p:val):mpred :=
   EX sh:_, 
   !!readable_share sh &&
   data_at sh sh (Tstruct _env_md_ctx_st noattr)
-*)*)
+*)*) *)
